theory/x64Assembler.thy
@@ -23,69 +23,113 @@ fun x64_encode :: "instruction \<Rightarrow> x64_bin option" where
     let (op:: u8) = 0xc1 in
     let (rop::u8) = construct_modsib_to_u8 0b11 0b000 (u8_of_ireg rd) in
     let (imm::u8) = ucast n in
-    if rex = 0 then
+    if rex = 0x40 then
       Some [prefix, op, rop, imm]
     else
-      let rex = bitfield_insert_u8 4 4 rex 0x4 in 
-        Some [prefix, rex, op, rop, imm] |
+      Some [prefix, rex, op, rop, imm] |
   \<comment> \<open> P2882 ` MOV: memory to reg`             ->  `0100 0RXB : 1000 101w : mod reg r/m`\<close>
   \<comment> \<open> P2882 ` MOV: memory64 to qwordregister` ->  `0100 1RXB : 1000 1011 : mod qwordreg r/m`\<close>
   Pmov_rm rd a c \<Rightarrow>( 
-      case a of Addrmode (Some rb) None z \<Rightarrow> (
-        let (rex::u8) = ( construct_rex_to_u8 \<comment> \<open> WRXB \<close>
-          (c = M64) \<comment> \<open> W \<close>
-          (and (u8_of_ireg rd) 0b1000 \<noteq> 0) \<comment> \<open> R \<close>
-          False \<comment> \<open> X \<close>
-          (and (u8_of_ireg rb) 0b1000 \<noteq> 0) \<comment> \<open> B \<close>
-          ) in
+    case a of Addrmode (Some rb) None dis \<Rightarrow> (
+      let (rex::u8) = ( construct_rex_to_u8 \<comment> \<open> WRXB \<close>
+        (c = M64) \<comment> \<open> W \<close>
+        (and (u8_of_ireg rd) 0b1000 \<noteq> 0) \<comment> \<open> R \<close>
+        False \<comment> \<open> X \<close>
+        (and (u8_of_ireg rb) 0b1000 \<noteq> 0) \<comment> \<open> B \<close>
+        ) in
+      if dis \<le> 127 \<or> dis \<ge> -128 then   \<comment> \<open> displacement8 : mod 01\<close>
+        let (dis::u8) = scast dis in
         let (rop::u8) = construct_modsib_to_u8 0b01 (u8_of_ireg rd) (u8_of_ireg rb) in
-          if (z \<le> 127) \<and> (z \<ge> -128) then   \<comment> \<open> displacement8 \<close>
-            let (dis::u8) = of_int z in
-            if rex = 0 then              
-              case c of 
-                M32 \<Rightarrow> Some [0x8b, rop, dis] |
-                M64 \<Rightarrow> Some [0x8b, rop, dis] |
-                _   \<Rightarrow> None
-            else 
-              let rex = bitfield_insert_u8 4 4 rex 0x4 in 
-                case c of 
-                  M32 \<Rightarrow> Some [rex, 0x8b, rop, dis] |
-                  M64 \<Rightarrow> Some [rex, 0x8b, rop, dis] |
-                  _   \<Rightarrow> None
-          else None)
-      | _ \<Rightarrow> None) 
-    |
+        if rex = 0x40 then    
+          case c of 
+            M32 \<Rightarrow> Some [0x8b, rop, dis] |
+            _   \<Rightarrow> None
+        else 
+          case c of 
+            M32 \<Rightarrow> Some [rex, 0x8b, rop, dis] |
+            M64 \<Rightarrow> Some [rex, 0x8b, rop, dis] |
+            _   \<Rightarrow> None
+      else if (and (u8_of_ireg rb) 0b0111 \<noteq> 0b100) then   \<comment> \<open> displacement8 : mod 10\<close>
+        let (rop::u8) = construct_modsib_to_u8 0b10 (u8_of_ireg rd) (u8_of_ireg rb) in
+          if rex = 0x40 then    
+            case c of 
+              M32 \<Rightarrow> Some ([0x8b, rop] @ (u8_list_of_u32 dis)) |
+              _   \<Rightarrow> None
+          else 
+            case c of 
+              M32 \<Rightarrow> Some ([rex, 0x8b, rop] @ (u8_list_of_u32 dis)) |
+              M64 \<Rightarrow> Some ([rex, 0x8b, rop] @ (u8_list_of_u32 dis)) |
+              _   \<Rightarrow> None  
+        else None)
+    |  Addrmode (Some rb) (Some (ri,scale)) dis \<Rightarrow>(
+        if scale > 3 | c \<noteq> M64 then None
+        else( 
+          let (rex::u8) = ( construct_rex_to_u8 \<comment> \<open> 1RXB \<close>
+            True \<comment> \<open> W \<close>
+            (and (u8_of_ireg rd) 0b1000 \<noteq> 0) \<comment> \<open> R \<close>
+            (and (u8_of_ireg ri) 0b1000 \<noteq> 0) \<comment> \<open> X \<close>
+            (and (u8_of_ireg rb) 0b1000 \<noteq> 0) \<comment> \<open> B \<close>
+            ) in
+          let (op:: u8) = 0x8b in
+          let (rop::u8) = construct_modsib_to_u8 0b10 (u8_of_ireg rd) 0b100 in
+          let (sib::u8) = construct_modsib_to_u8 scale (u8_of_ireg ri) (u8_of_ireg rb) in
+            Some ([rex, op, rop, sib] @ (u8_list_of_u32 dis))))
+    | _ \<Rightarrow> None) 
+  |
   \<comment> \<open> P2882 ` MOV: reg to memory`             ->  `0100 0RXB : 1000 1000 : mod reg r/m `\<close>
   \<comment> \<open> P2882 ` MOV: reg to memory`             ->  `66H 0100 0RXB : 1000 1001 : mod reg r/m `\<close>
   \<comment> \<open> P2882 ` MOV: reg to memory`             ->  `0100 0RXB : 1000 1001 : mod reg r/m` \<close>
   \<comment> \<open> P2882 ` MOV: qwordregister to memory64` ->  `0100 1RXB 1000 1001 : mod qwordreg r/m` \<close>
-  Pmov_mr  a r1 c \<Rightarrow> 
-    if r1 = R10 then 
-      case a of Addrmode (Some rd) None z \<Rightarrow> 
-        let (rex::u8) = ( construct_rex_to_u8 \<comment> \<open> WRXB \<close>
-          (c = M64) \<comment> \<open> W \<close>
-          (and (u8_of_ireg r1) 0b1000 \<noteq> 0) \<comment> \<open> R \<close>
-          False \<comment> \<open> X \<close>
-          (and (u8_of_ireg rd) 0b1000 \<noteq> 0) \<comment> \<open> B \<close>
-          ) in
-        let (rop::u8) = construct_modsib_to_u8 0b01 (u8_of_ireg r1) (u8_of_ireg rd) in
-        if (z \<le> 127) \<and> (z \<ge> -128) then   \<comment> \<open> displacement8 \<close>
-          let (dis::u8) = of_int z in
-          if rex = 0 then
-            case c of 
-              M8  \<Rightarrow> Some [0x88, rop, dis] |
-              M16 \<Rightarrow> Some [0x66, 0x89, rop, dis] |
-              M32 \<Rightarrow> Some [0x89, rop, dis] |
-              M64 \<Rightarrow> Some [0x89, rop, dis]
-          else 
-            case c of 
-              M8  \<Rightarrow> Some [rex, 0x88, rop, dis] |
-              M16 \<Rightarrow> Some [0x66,rex, 0x89, rop, dis] |
-              M32 \<Rightarrow> Some [rex, 0x89, rop, dis] |
-              M64 \<Rightarrow> Some [rex, 0x89, rop, dis]
+  Pmov_mr  a r1 c \<Rightarrow> (
+    case a of Addrmode (Some rb) None dis \<Rightarrow> 
+      let (rex::u8) = ( construct_rex_to_u8 \<comment> \<open> WRXB \<close>
+        (c = M64) \<comment> \<open> W \<close>
+        (and (u8_of_ireg r1) 0b1000 \<noteq> 0) \<comment> \<open> R \<close>
+        False \<comment> \<open> X \<close>
+        (and (u8_of_ireg rb) 0b1000 \<noteq> 0) \<comment> \<open> B \<close>
+        ) in
+      if dis \<le> 127 \<or> dis \<ge> -128  then   \<comment> \<open> displacement8 : mod 01 \<close>
+        let (dis::u8) = scast dis in
+        let (rop::u8) = construct_modsib_to_u8 0b01 (u8_of_ireg r1) (u8_of_ireg rb) in
+        if rex = 0x40 then(
+          case c of 
+            M8  \<Rightarrow> Some [0x88, rop, dis] |
+            M16 \<Rightarrow> Some [0x66, 0x89, rop, dis] |
+            M32 \<Rightarrow> Some [0x89, rop, dis] |
+            _   \<Rightarrow> None)
+        else (
+          case c of 
+            M8  \<Rightarrow> Some [rex, 0x88, rop, dis] |
+            M16 \<Rightarrow> Some [0x66,rex, 0x89, rop, dis] |
+            M32 \<Rightarrow> Some [rex, 0x89, rop, dis] |
+            M64 \<Rightarrow> Some [rex, 0x89, rop, dis])
+      else if (and (u8_of_ireg rb) 0b0111 \<noteq> 0b100) then   \<comment> \<open> displacement8 : mod 10\<close>       
+        let (rop::u8) = construct_modsib_to_u8 0b10 (u8_of_ireg r1) (u8_of_ireg rb) in
+        if rex = 0x40 then(
+          case c of 
+            M32 \<Rightarrow> Some ([0x89, rop] @ (u8_list_of_u32 dis)) |
+            _   \<Rightarrow> None)
+        else (
+          case c of 
+            M32 \<Rightarrow> Some ([rex, 0x89, rop] @ (u8_list_of_u32 dis)) |
+            M64 \<Rightarrow> Some ([rex, 0x89, rop] @ (u8_list_of_u32 dis)) |
+            _   \<Rightarrow> None)
         else None
-      | _ \<Rightarrow> None 
-    else None |
+    |  Addrmode (Some rb) (Some (ri,scale)) dis \<Rightarrow>
+        if scale > 3 | c \<noteq> M64 then None
+        else 
+          let (rex::u8) = ( construct_rex_to_u8 \<comment> \<open> 1RXB \<close>
+            True \<comment> \<open> W \<close>
+            (and (u8_of_ireg r1) 0b1000 \<noteq> 0) \<comment> \<open> R \<close>
+            (and (u8_of_ireg ri) 0b1000 \<noteq> 0) \<comment> \<open> X \<close>
+            (and (u8_of_ireg rb) 0b1000 \<noteq> 0) \<comment> \<open> B \<close>
+            ) in
+        let (op:: u8) = 0x89 in
+        let (rop::u8) = construct_modsib_to_u8 0b10 (u8_of_ireg r1) 0b100 in
+        let (sib::u8) = construct_modsib_to_u8 scale (u8_of_ireg ri) (u8_of_ireg rb) in
+            Some ([rex, op, rop, sib] @ (u8_list_of_u32 dis))
+    | _ \<Rightarrow> None) 
+  |
   \<comment> \<open> P2887 `MOV register1 to register2` -> `0100 0R0B : 1000 1001 : 11 reg1 reg2` \<close>
   Pmovl_rr rd r1 \<Rightarrow>
     let (rex::u8) = ( construct_rex_to_u8 \<comment> \<open> `0R0B` \<close>
@@ -96,11 +140,10 @@ fun x64_encode :: "instruction \<Rightarrow> x64_bin option" where
       ) in
     let (op:: u8) = 0x89 in
     let (rop::u8) = construct_modsib_to_u8 0b11 (u8_of_ireg r1) (u8_of_ireg rd) in
-    if rex = 0 then
+    if rex = 0x40 then
       Some [op, rop]
     else
-      let rex = bitfield_insert_u8 4 4 rex 0x4 in 
-        Some [rex, op, rop] |
+      Some [rex, op, rop] |
   \<comment> \<open> P2882 `MOV qwordregister1 to qwordregister2` -> `0100 1R0B : 1000 1001 : 11 reg1 reg2` \<close>
   Pmovq_rr rd r1 \<Rightarrow>
     let (rex:: u8) = (construct_rex_to_u8  \<comment> \<open> `1R0B` \<close>
@@ -111,7 +154,6 @@ fun x64_encode :: "instruction \<Rightarrow> x64_bin option" where
       ) in
     let (op:: u8) = 0x89 in
     let (rop::u8) = construct_modsib_to_u8 0b11 (u8_of_ireg r1) (u8_of_ireg rd) in
-    let rex = bitfield_insert_u8 4 4 rex 0x4 in
       Some [ rex, op, rop ] |
   \<comment> \<open> P2882 `MOV immediate to register` -> `0100 000B : 1100 011w : 11 000 reg : imm` \<close>
   Pmovl_ri rd n \<Rightarrow>
@@ -123,11 +165,10 @@ fun x64_encode :: "instruction \<Rightarrow> x64_bin option" where
       ) in
     let (op:: u8) = 0xc7 in
     let (rop::u8) = construct_modsib_to_u8 0b11 0b000 (u8_of_ireg rd) in
-      if rex = 0 then
+      if rex = 0x40 then
         Some ([op, rop] @ (u8_list_of_u32 n))
       else
-        let rex = bitfield_insert_u8 4 4 rex 0x4 in 
-          Some ([rex, op, rop] @ (u8_list_of_u32 n)) |
+        Some ([rex, op, rop] @ (u8_list_of_u32 n)) |
   \<comment> \<open> P2882 `MOV immediate64 to qwordregister (alternate encoding)` -> `0100 100B 1011 1reg : imm64` \<close>
   Pmovq_ri rd n \<Rightarrow>
     let (rex::u8) = ( construct_rex_to_u8 \<comment> \<open> `100B` \<close>
@@ -136,19 +177,64 @@ fun x64_encode :: "instruction \<Rightarrow> x64_bin option" where
       False \<comment> \<open> X \<close>
       (and (u8_of_ireg rd) 0b1000 \<noteq> 0) \<comment> \<open> B \<close>
       ) in
-    let (op:: u8) = or 0xb8 (and (u8_of_ireg rd) 0b111 ) in
+    let (op:: u8) = bitfield_insert_u8 0 3 0xb8 (u8_of_ireg rd) in
       Some ([rex, op] @ u8_list_of_u64 n)|
+  \<comment> \<open> P2882 `MOV immediate32 to memory64 (zero extend)` -> ` 0100 10XB 1100 0111 : mod 000 r/m : imm32` \<close>
+  Pmov_mi a n M64 \<Rightarrow>(
+    case a of Addrmode (Some rd) None dis \<Rightarrow>( 
+      let (rex:: u8) = (construct_rex_to_u8  \<comment> \<open> `100B` \<close>
+        True \<comment> \<open> W \<close>
+        False \<comment> \<open> R \<close>
+        False \<comment> \<open> X \<close>
+        (and (u8_of_ireg rd) 0b1000 \<noteq> 0) \<comment> \<open> B \<close>
+        ) in
+      let (op:: u8) = 0xc7 in
+        if dis \<le> 127 \<or> dis \<ge> -128  then   \<comment> \<open> displacement8 : mod 01 \<close>
+          let (dis::u8) = scast dis in
+          let (rop::u8) = construct_modsib_to_u8 0b01 0b000 (u8_of_ireg rd) in
+            Some ([ rex, op, rop, dis ] @ (u8_list_of_u32 n))
+        else  \<comment> \<open> displacement32 : mod 10 \<close>
+          let (rop::u8) = construct_modsib_to_u8 0b10 0b000 (u8_of_ireg rd) in
+            Some ([ rex, op, rop ] @ (u8_list_of_u32 dis) @ (u8_list_of_u32 n)) )
+    | _\<Rightarrow> None) |
   \<comment> \<open> P2883 `MOVXD dwordregister2 to qwordregister1` -> ` 0100 1R0B 0110 0011 : 11 quadreg1 dwordreg2` \<close>
   Pmovsq_rr rd r1 \<Rightarrow>
     let (rex:: u8) = (construct_rex_to_u8  \<comment> \<open> `1R0B` \<close>
       True \<comment> \<open> W \<close>
-      (and (u8_of_ireg r1) 0b1000 \<noteq> 0) \<comment> \<open> R \<close>
+      (and (u8_of_ireg rd) 0b1000 \<noteq> 0) \<comment> \<open> R \<close>
       False \<comment> \<open> X \<close>
-      (and (u8_of_ireg rd) 0b1000 \<noteq> 0) \<comment> \<open> B \<close>
+      (and (u8_of_ireg r1) 0b1000 \<noteq> 0) \<comment> \<open> B \<close>
       ) in
     let (op:: u8) = 0x63 in
     let (rop::u8) = construct_modsib_to_u8 0b11 (u8_of_ireg rd) (u8_of_ireg r1) in
       Some [ rex, op, rop ] |
+  \<comment> \<open> P2919 `MOVcc : resgister2  to resgister1 ` -> `0100 0R0B 0000 1111: 0100 tttn : 11 reg1 reg2` \<close>
+  Pcmovl t rd r1 \<Rightarrow>
+    let (rex::u8) = ( construct_rex_to_u8 \<comment> \<open> `0R0B` \<close>
+      False \<comment> \<open> W \<close>
+      (and (u8_of_ireg rd) 0b1000 \<noteq> 0) \<comment> \<open> R \<close>
+      False \<comment> \<open> X \<close>
+      (and (u8_of_ireg r1) 0b1000 \<noteq> 0) \<comment> \<open> B \<close>
+      ) in
+    let (ex:: u8) = 0x0f in
+    let (op:: u8) = bitfield_insert_u8 0 4 0x40 (u8_of_cond t) in   \<comment> \<open> 45 : NZ/NE （ZF=0 \<close>   
+    let (rop::u8) = construct_modsib_to_u8 0b11 (u8_of_ireg rd) (u8_of_ireg r1) in
+    if rex = 0x40 then
+      Some [ex, op, rop]
+    else
+      Some [rex, ex, op, rop] |
+  \<comment> \<open> P2919 `MOVcc : qwordregister2 to qwordregister1` -> ` 0100 1R0B 0000 1111: 0100 tttn : 11 qwordreg1 qwordreg2` \<close>
+  Pcmovq t rd r1 \<Rightarrow>
+    let (rex:: u8) = (construct_rex_to_u8  \<comment> \<open> `1R0B` \<close>
+      True \<comment> \<open> W \<close>
+      (and (u8_of_ireg rd) 0b1000 \<noteq> 0) \<comment> \<open> R \<close>
+      False \<comment> \<open> X \<close>
+      (and (u8_of_ireg r1) 0b1000 \<noteq> 0) \<comment> \<open> B \<close>
+      ) in
+    let (ex:: u8) = 0x0f in
+    let (op:: u8) = bitfield_insert_u8 0 4 0x40 (u8_of_cond t) in  \<comment> \<open> 45 : NZ/NE （ZF=0 \<close> 
+    let (rop::u8) = construct_modsib_to_u8 0b11 (u8_of_ireg rd) (u8_of_ireg r1) in
+      Some [rex, ex, op, rop] |
   \<comment> \<open> P2893 `XCHG: register1 with register2 `   -> ` 0100 1R0B 1000 011w : 11 reg1 reg2 ` \<close>
   Pxchgq_rr rd r1 \<Rightarrow>
     let (rex:: u8) = (construct_rex_to_u8  \<comment> \<open> `1R0B` \<close>
@@ -160,17 +246,29 @@ fun x64_encode :: "instruction \<Rightarrow> x64_bin option" where
     let (op::u8) = 0x87 in
     let (rop::u8) = construct_modsib_to_u8 0b11 (u8_of_ireg r1) (u8_of_ireg rd) in
       Some [rex, op, rop] |
-  \<comment> \<open> P2882 `MOV immediate32 to memory64 (zero extend)` -> ` 0100 10XB 1100 0111 : mod 000 r/m : imm32` 
-  Pmovq_ri rd n \<Rightarrow>
-    let (rex:: u8) = (construct_rex_to_u8  \<comment> \<open> `1R0B` \<close>
-      True \<comment> \<open> W \<close>
-      False \<comment> \<open> R \<close>
-      True \<comment> \<open> X \<close>
-      (and (u8_of_ireg rd) 0b1000 \<noteq> 0) \<comment> \<open> B \<close>
-      ) in
-    let (op:: u8) = 0xc7 in
-    let (rop::u8) = construct_modsib_to_u8 0b01 0b000 (u8_of_ireg rd) in
-      Some [ rex, op, rop ] |   \<close>
+  \<comment> \<open> P2893 `XCHG: memory64 with qwordregister `   -> ` 0100 1R0B 1000 011w : 11 reg1 reg2 ` \<close>
+  Pxchgq_rm r1 a M64 \<Rightarrow>( 
+    case a of Addrmode (Some rb) (Some (ri,scale)) dis \<Rightarrow>(
+      if scale > 3 then None
+      else 
+        let (rex:: u8) = (construct_rex_to_u8  \<comment> \<open> `1RXB` \<close>
+          True \<comment> \<open> W \<close>
+          (and (u8_of_ireg r1) 0b1000 \<noteq> 0) \<comment> \<open> R \<close>
+          (and (u8_of_ireg ri) 0b1000 \<noteq> 0) \<comment> \<open> X \<close>
+          (and (u8_of_ireg rb) 0b1000 \<noteq> 0) \<comment> \<open> B \<close>
+          ) in
+        let (op:: u8) = 0x87 in
+        let (rop::u8) = construct_modsib_to_u8 0b10 (u8_of_ireg r1) 0b100 in
+        let (sib::u8) = construct_modsib_to_u8 scale (u8_of_ireg ri) (u8_of_ireg rb) in
+            Some ([rex, op, rop, sib] @ (u8_list_of_u32 dis))
+      ) |
+      _ \<Rightarrow> None)|
+  \<comment> \<open> P2878 `CDQ : sign_extend_eax_edx `   -> ` 1001 1001 ` \<close>  
+  Pcdq \<Rightarrow>
+    Some [0x99] |
+  \<comment> \<open> P2878 `CQO : sign_extend_rax_rdx `   -> ` 0100 1001 1001 1001 ` \<close>
+  Pcqo \<Rightarrow>
+    Some [0x48, 0x99] |
   \<comment> \<open> P2876 `ADD register1 to register2` -> `0100 0R0B : 0000 000w : 11 reg1 reg2` \<close>
   Paddl_rr rd r1 \<Rightarrow>
     let (rex:: u8) = (construct_rex_to_u8  \<comment> \<open> `0R0B` \<close>
@@ -181,10 +279,9 @@ fun x64_encode :: "instruction \<Rightarrow> x64_bin option" where
       ) in
     let (op:: u8) = 0x01 in
     let (rop::u8) = construct_modsib_to_u8 0b11 (u8_of_ireg r1) (u8_of_ireg rd) in
-      if rex = 0 then
+      if rex = 0x40 then
         Some [ op, rop ] 
       else 
-      let rex = bitfield_insert_u8 4 4 rex 0x4 in 
         Some [ rex, op, rop ] |
  \<comment> \<open> P2876 `ADD immediate to register` -> `0100 000B : 1000 00sw : 11 000 reg : immediate data` \<close>
   Paddl_ri rd n \<Rightarrow>
@@ -194,13 +291,26 @@ fun x64_encode :: "instruction \<Rightarrow> x64_bin option" where
       False \<comment> \<open> X \<close>
       (and (u8_of_ireg rd) 0b1000 \<noteq> 0) \<comment> \<open> B \<close>
       ) in
-    let (op:: u8) = 0x01 in
+    let (op:: u8) = 0x81 in
     let (rop::u8) = construct_modsib_to_u8 0b11 0b000 (u8_of_ireg rd) in
-    if rex = 0 then
+    if rex = 0x40 then
       Some ([op, rop] @ u8_list_of_u32 n) 
     else 
-      let rex = bitfield_insert_u8 4 4 rex 0x4 in 
-        Some  ([rex, op, rop] @ u8_list_of_u32 n) |
+      Some  ([rex, op, rop] @ u8_list_of_u32 n) |
+ \<comment> \<open> P2876 `ADD imm16 to reg16` -> `0x66 0100 000B : 1000 00sw : 11 000 reg : imm16` \<close>
+  Paddw_ri rd n \<Rightarrow>
+    let (rex:: u8) = (construct_rex_to_u8  \<comment> \<open> `000B` \<close>
+      False \<comment> \<open> W \<close>
+      False \<comment> \<open> R \<close>
+      False \<comment> \<open> X \<close>
+      (and (u8_of_ireg rd) 0b1000 \<noteq> 0) \<comment> \<open> B \<close>
+      ) in
+    let (op:: u8) = 0x81 in
+    let (rop::u8) = construct_modsib_to_u8 0b11 0b000 (u8_of_ireg rd) in
+    if rex = 0x40 then
+      Some ([0x66, op, rop] @ u8_list_of_u16 n) 
+    else 
+      Some  ([0x66, rex, op, rop] @ u8_list_of_u16 n) |
   \<comment> \<open> P2876 `ADD qwordregister1 to qwordregister2` -> `0100 1R0B : 0000 0001 : 11 reg1 reg2` \<close>
   Paddq_rr rd r1 \<Rightarrow>
     let (rex:: u8) = (construct_rex_to_u8  \<comment> \<open> `1R0B` \<close>
@@ -212,6 +322,23 @@ fun x64_encode :: "instruction \<Rightarrow> x64_bin option" where
     let (op:: u8) = 0x01 in
     let (rop::u8) = construct_modsib_to_u8 0b11 (u8_of_ireg r1) (u8_of_ireg rd) in
       Some [ rex, op, rop ] |
+  \<comment> \<open> P2876 `ADD immediate32 to memory64` -> ` 0100 10XB : 1000 0001 : mod 000 r/m : imm32` \<close>
+  Paddq_mi a n M64 \<Rightarrow>( 
+    case a of Addrmode (Some rb) (Some (ri,scale)) dis \<Rightarrow>(
+      if scale > 3 then None
+      else 
+        let (rex:: u8) = (construct_rex_to_u8  \<comment> \<open> `10XB` \<close>
+          True \<comment> \<open> W \<close>
+          False \<comment> \<open> R \<close>
+          (and (u8_of_ireg ri) 0b1000 \<noteq> 0) \<comment> \<open> X \<close>
+          (and (u8_of_ireg rb) 0b1000 \<noteq> 0) \<comment> \<open> B \<close>
+          ) in
+        let (op:: u8) = 0x81 in
+        let (rop::u8) = construct_modsib_to_u8 0b10 0b000 0b100 in
+        let (sib::u8) = construct_modsib_to_u8 scale (u8_of_ireg ri) (u8_of_ireg rb) in
+            Some ([rex, op, rop, sib] @ (u8_list_of_u32 dis) @ (u8_list_of_u32 n))
+      ) |
+      _ \<Rightarrow> None)|
   \<comment> \<open> P2891 `SUB register1 from register2` -> `0100 0R0B : 0010 100w : 11 reg1 reg2` \<close>
   Psubl_rr rd r1 \<Rightarrow>
     let (rex:: u8) = (construct_rex_to_u8  \<comment> \<open> `0R0B` \<close>
@@ -222,7 +349,10 @@ fun x64_encode :: "instruction \<Rightarrow> x64_bin option" where
       ) in
     let (op:: u8) = 0x29 in
     let (rop::u8) = construct_modsib_to_u8 0b11 (u8_of_ireg r1) (u8_of_ireg rd) in
-      Some [ rex, op, rop ] |
+      if rex = 0x40 then
+        Some [ op, rop ] 
+      else 
+        Some [ rex, op, rop ] |
   \<comment> \<open> P2891 `SUB qwordregister1 from qwordregister2` -> `0100 1R0B : 0010 1001 : 11 reg1 reg2` \<close>
   Psubq_rr rd r1 \<Rightarrow>
     let (rex:: u8) = (construct_rex_to_u8  \<comment> \<open> `1R0B` \<close>
@@ -244,7 +374,24 @@ fun x64_encode :: "instruction \<Rightarrow> x64_bin option" where
       ) in
     let (op:: u8) = 0xf7 in
     let (rop::u8) = construct_modsib_to_u8 0b11 0b011 (u8_of_ireg rd) in
-      Some [rex, op, rop ] |
+      if rex = 0x40 then
+        Some [ op, rop ] 
+      else 
+        Some [ rex, op, rop ] |
+ \<comment> \<open> P2891 `SUB: immediate from register` -> `0100 000B 1000 00sw : 11 101 reg : imm` \<close>
+  Psubl_ri rd n \<Rightarrow>
+    let (rex:: u8) = (construct_rex_to_u8  \<comment> \<open> `000B` \<close>
+      False \<comment> \<open> W \<close>
+      False \<comment> \<open> R \<close>
+      False \<comment> \<open> X \<close>
+      (and (u8_of_ireg rd) 0b1000 \<noteq> 0) \<comment> \<open> B \<close>
+      ) in
+    let (op:: u8) = 0x81 in
+    let (rop::u8) = construct_modsib_to_u8 0b11 0b101 (u8_of_ireg rd) in
+      if rex = 0x40 then
+        Some ([op, rop] @ u8_list_of_u32 n) 
+      else 
+        Some  ([rex, op, rop] @ u8_list_of_u32 n) |
   \<comment> \<open> P2884 `NEG register2` -> `0100 100B : 1111 0111 : 11011reg` \<close>
   Pnegq rd \<Rightarrow>
     let (rex:: u8) = (construct_rex_to_u8  \<comment> \<open> `100B` \<close>
@@ -258,7 +405,7 @@ fun x64_encode :: "instruction \<Rightarrow> x64_bin option" where
       Some [rex, op, rop ] |
   \<comment> \<open> P2884 `OR register1 to register2` -> ` 0000 100w : 11 reg1 reg2` \<close>
   Porl_rr rd r1  \<Rightarrow> 
-     let (rex:: u8) = (construct_rex_to_u8  \<comment> \<open> `1R0B` \<close>
+     let (rex:: u8) = (construct_rex_to_u8  \<comment> \<open> `0R0B` \<close>
       False \<comment> \<open> W \<close>
       (and (u8_of_ireg r1) 0b1000 \<noteq> 0) \<comment> \<open> R \<close>
       False \<comment> \<open> X \<close>
@@ -266,7 +413,10 @@ fun x64_encode :: "instruction \<Rightarrow> x64_bin option" where
       ) in
     let (op:: u8) = 0x09 in
     let (rop::u8) = construct_modsib_to_u8 0b11 (u8_of_ireg r1) (u8_of_ireg rd) in
-      Some [ rex, op, rop ] |
+      if rex = 0x40 then
+        Some [ op, rop ] 
+      else 
+        Some [ rex, op, rop ] |
   \<comment> \<open> P2884 `OR qwordregister1 to qwordregister2` -> ` 0100 1R0B : 0000 1001 : 11 reg1 reg2` \<close>
   Porq_rr rd r1  \<Rightarrow> 
      let (rex:: u8) = (construct_rex_to_u8  \<comment> \<open> `1R0B` \<close>
@@ -278,6 +428,20 @@ fun x64_encode :: "instruction \<Rightarrow> x64_bin option" where
     let (op:: u8) = 0x09 in
     let (rop::u8) = construct_modsib_to_u8 0b11 (u8_of_ireg r1) (u8_of_ireg rd) in
       Some [ rex, op, rop] |
+ \<comment> \<open> P2891 `OR: immediate to register` -> `0100 000B  1000 00sw : 11 001 reg : imm` \<close>
+  Porl_ri rd n \<Rightarrow>
+    let (rex:: u8) = (construct_rex_to_u8  \<comment> \<open> `000B` \<close>
+      False \<comment> \<open> W \<close>
+      False \<comment> \<open> R \<close>
+      False \<comment> \<open> X \<close>
+      (and (u8_of_ireg rd) 0b1000 \<noteq> 0) \<comment> \<open> B \<close>
+      ) in
+    let (op:: u8) = 0x81 in
+    let (rop::u8) = construct_modsib_to_u8 0b11 0b001 (u8_of_ireg rd) in
+      if rex = 0x40 then
+        Some ([op, rop] @ u8_list_of_u32 n) 
+      else 
+        Some  ([rex, op, rop] @ u8_list_of_u32 n) |
   \<comment> \<open> P2876 `AND register1 to register2` -> ` 0100 0R0B : 0010 000w : 11 reg1 reg2` \<close>
   Pandl_rr rd r1  \<Rightarrow> 
      let (rex:: u8) = (construct_rex_to_u8  \<comment> \<open> `0R0B` \<close>
@@ -288,7 +452,10 @@ fun x64_encode :: "instruction \<Rightarrow> x64_bin option" where
       ) in
     let (op:: u8) = 0x21 in
     let (rop::u8) = construct_modsib_to_u8 0b11 (u8_of_ireg r1) (u8_of_ireg rd) in
-      Some [ rex, op, rop] |
+      if rex = 0x40 then
+        Some [ op, rop ] 
+      else 
+        Some [ rex, op, rop ] |
   \<comment> \<open> P2876 `AND qwordregister1 to qwordregister2` -> ` 0100 1R0B : 0010 0001 : 11 reg1 reg2` \<close>
   Pandq_rr rd r1  \<Rightarrow> 
      let (rex:: u8) = (construct_rex_to_u8  \<comment> \<open> `1R0B` \<close>
@@ -300,6 +467,20 @@ fun x64_encode :: "instruction \<Rightarrow> x64_bin option" where
     let (op:: u8) = 0x21 in
     let (rop::u8) = construct_modsib_to_u8 0b11 (u8_of_ireg r1) (u8_of_ireg rd) in
       Some [ rex, op, rop] |
+ \<comment> \<open> P2891 `AND: immediate to register` -> `0100 000B : 1000 00sw : 11 100 reg : immediate` \<close>
+  Pandl_ri rd n \<Rightarrow>
+    let (rex:: u8) = (construct_rex_to_u8  \<comment> \<open> `000B` \<close>
+      False \<comment> \<open> W \<close>
+      False \<comment> \<open> R \<close>
+      False \<comment> \<open> X \<close>
+      (and (u8_of_ireg rd) 0b1000 \<noteq> 0) \<comment> \<open> B \<close>
+      ) in
+    let (op:: u8) = 0x81 in
+    let (rop::u8) = construct_modsib_to_u8 0b11 0b100 (u8_of_ireg rd) in
+      if rex = 0x40 then
+        Some ([op, rop] @ u8_list_of_u32 n) 
+      else 
+        Some  ([rex, op, rop] @ u8_list_of_u32 n) |
   \<comment> \<open> P2893 `XOR register1 to register2` -> ` 0100 0RXB : 0011 000w : 11 reg1 reg2` \<close>
   Pxorl_rr rd r1  \<Rightarrow> 
      let (rex:: u8) = (construct_rex_to_u8  \<comment> \<open> `0R0B` \<close>
@@ -310,7 +491,10 @@ fun x64_encode :: "instruction \<Rightarrow> x64_bin option" where
       ) in
     let (op:: u8) = 0x31 in
     let (rop::u8) = construct_modsib_to_u8 0b11 (u8_of_ireg r1) (u8_of_ireg rd) in
-      Some [ rex, op, rop] |
+      if rex = 0x40 then
+        Some [ op, rop ] 
+      else 
+        Some [ rex, op, rop ] |
   \<comment> \<open> P2893 `XOR qwordregister1 to qwordregister2` -> ` 0100 1R0B : 0011 0001 : 11 reg1 reg2` \<close>
   Pxorq_rr rd r1  \<Rightarrow> 
      let (rex:: u8) = (construct_rex_to_u8  \<comment> \<open> `1R0B` \<close>
@@ -322,6 +506,20 @@ fun x64_encode :: "instruction \<Rightarrow> x64_bin option" where
     let (op:: u8) = 0x31 in
     let (rop::u8) = construct_modsib_to_u8 0b11 (u8_of_ireg r1) (u8_of_ireg rd) in
       Some [ rex, op, rop] |
+  \<comment> \<open> P2893 `XOR: immediate to register` -> ` 0100 000B 1000 00sw : 11 110 reg : imm` \<close>
+  Pxorl_ri rd n \<Rightarrow>
+    let (rex:: u8) = (construct_rex_to_u8  \<comment> \<open> `000B` \<close>
+      False \<comment> \<open> W \<close>
+      False \<comment> \<open> R \<close>
+      False \<comment> \<open> X \<close>
+      (and (u8_of_ireg rd) 0b1000 \<noteq> 0) \<comment> \<open> B \<close>
+      ) in
+    let (op:: u8) = 0x81 in
+    let (rop::u8) = construct_modsib_to_u8 0b11 0b110 (u8_of_ireg rd) in
+      if rex = 0x40 then
+        Some ([op, rop] @ u8_list_of_u32 n) 
+      else 
+        Some  ([rex, op, rop] @ u8_list_of_u32 n) |
   \<comment> \<open> P2884 `MUL AL, AX, or EAX with register2` -> ` 0100 000B : 1111 011w : 11 100 reg` \<close>
   Pmull_r r1 \<Rightarrow>
     let (rex:: u8) = (construct_rex_to_u8  \<comment> \<open> `000B` \<close>
@@ -332,7 +530,10 @@ fun x64_encode :: "instruction \<Rightarrow> x64_bin option" where
       ) in
     let (op:: u8) = 0xf7 in
     let (rop::u8) = construct_modsib_to_u8 0b11 0b100 (u8_of_ireg r1) in
-      Some [ rex, op, rop] |
+      if rex = 0x40 then
+        Some [ op, rop ] 
+      else 
+        Some [ rex, op, rop ] |
   \<comment> \<open> P2884 `MUL RAX with qwordregister (to RDX:RAX)` -> ` 0100 100B : 1111 0111 : 11 100 qowrdreg` \<close>
   Pmulq_r r1 \<Rightarrow>
     let (rex:: u8) = (construct_rex_to_u8  \<comment> \<open> `100B` \<close>
@@ -354,7 +555,10 @@ fun x64_encode :: "instruction \<Rightarrow> x64_bin option" where
       ) in
     let (op:: u8) = 0xf7 in
     let (rop::u8) = construct_modsib_to_u8 0b11 0b101 (u8_of_ireg r1) in
-      Some [ rex, op, rop] |
+      if rex = 0x40 then
+        Some [ op, rop ] 
+      else 
+        Some [ rex, op, rop ] |
   \<comment> \<open> P2880 `IMUL RAX with qwordregister (to RDX:RAX)` -> ` 0100 100B : 1111 0111 : 11 101 qwordreg` \<close>
   Pimulq_r r1 \<Rightarrow>
     let (rex:: u8) = (construct_rex_to_u8  \<comment> \<open> `100B` \<close>
@@ -376,7 +580,10 @@ fun x64_encode :: "instruction \<Rightarrow> x64_bin option" where
       ) in
     let (op:: u8) = 0xf7 in
     let (rop::u8) = construct_modsib_to_u8 0b11 0b110 (u8_of_ireg r1) in
-      Some [ rex, op, rop] |
+      if rex = 0x40 then
+        Some [ op, rop ] 
+      else 
+        Some [ rex, op, rop ] |
   \<comment> \<open> P2879 `DIV EAX by qwordregister (to RDX:RAX)` -> ` 0100 100B : 1111 0111 : 11 110 qwordreg` \<close>
   Pdivq_r r1 \<Rightarrow>
     let (rex:: u8) = (construct_rex_to_u8  \<comment> \<open> `100B` \<close>
@@ -398,7 +605,10 @@ fun x64_encode :: "instruction \<Rightarrow> x64_bin option" where
       ) in
     let (op:: u8) = 0xf7 in
     let (rop::u8) = construct_modsib_to_u8 0b11 0b111 (u8_of_ireg r1) in
-      Some [ rex, op, rop] |
+      if rex = 0x40 then
+        Some [ op, rop ] 
+      else 
+        Some [ rex, op, rop ] |
   \<comment> \<open> P2879 `IDIV RAX by qwordregister (to RDX:RAX)` -> ` 0100 100B : 1111 0111 : 11 111 qwordreg` \<close>
   Pidivq_r r1 \<Rightarrow>
     let (rex:: u8) = (construct_rex_to_u8  \<comment> \<open> `100B` \<close>
@@ -421,7 +631,10 @@ fun x64_encode :: "instruction \<Rightarrow> x64_bin option" where
     let (op:: u8) = 0xc1 in
     let (rop::u8) = construct_modsib_to_u8 0b11 0b100 (u8_of_ireg rd) in
     let (imm::u8) = ucast n in
-      Some [ rex, op, rop, imm] |
+      if rex = 0x40 then
+        Some [ op, rop, imm ] 
+      else 
+        Some [ rex, op, rop, imm ] |
   \<comment> \<open> P2889 `SHL qwordregister by immediate count` -> ` 0100 100B 1100 0001 : 11 100 reg : imm8 ` \<close>
   Pshlq_ri rd n \<Rightarrow>
     let (rex:: u8) = (construct_rex_to_u8  \<comment> \<open> `100B` \<close>
@@ -433,7 +646,7 @@ fun x64_encode :: "instruction \<Rightarrow> x64_bin option" where
     let (op:: u8) = 0xc1 in
     let (rop::u8) = construct_modsib_to_u8 0b11 0b100 (u8_of_ireg rd) in
     let (imm::u8) = ucast n in
-      Some [ rex, op, rop, imm] |
+      Some [ rex, op, rop, imm ] |
   \<comment> \<open> P2889 `SHL register by CL`                   -> ` 0100 000B 1101 001w : 11 100 reg ` \<close>
   Pshll_r rd  \<Rightarrow>
     let (rex:: u8) = (construct_rex_to_u8  \<comment> \<open> `000B` \<close>
@@ -444,7 +657,10 @@ fun x64_encode :: "instruction \<Rightarrow> x64_bin option" where
       ) in
     let (op:: u8) = 0xd3 in
     let (rop::u8) = construct_modsib_to_u8 0b11 0b100 (u8_of_ireg rd) in
-      Some [ rex, op, rop] |
+      if rex = 0x40 then
+        Some [ op, rop ] 
+      else 
+        Some [ rex, op, rop ] |
   \<comment> \<open> P2889 `SHL qwordregister by CL`              -> ` 0100 100B 1101 001w : 11 100 reg ` \<close>
   Pshlq_r rd  \<Rightarrow>
     let (rex:: u8) = (construct_rex_to_u8  \<comment> \<open> `100B` \<close>
@@ -467,7 +683,10 @@ fun x64_encode :: "instruction \<Rightarrow> x64_bin option" where
     let (op:: u8) = 0xc1 in
     let (rop::u8) = construct_modsib_to_u8 0b11 0b101 (u8_of_ireg rd) in
     let (imm::u8) = ucast n in
-      Some [ rex, op, rop, imm] |
+      if rex = 0x40 then
+        Some [ op, rop, imm ] 
+      else 
+        Some [ rex, op, rop, imm ] |
   \<comment> \<open> P2890 `SHR qwordregister by immediate count` -> ` 0100 100B 1100 000w : 11 101 reg : imm8 ` \<close>
   Pshrq_ri rd n \<Rightarrow>
     let (rex:: u8) = (construct_rex_to_u8  \<comment> \<open> `100B` \<close>
@@ -490,7 +709,10 @@ fun x64_encode :: "instruction \<Rightarrow> x64_bin option" where
       ) in
     let (op:: u8) = 0xd3 in
     let (rop::u8) = construct_modsib_to_u8 0b11 0b101 (u8_of_ireg rd) in
-      Some [ rex, op, rop ] |
+      if rex = 0x40 then
+        Some [ op, rop ] 
+      else 
+        Some [ rex, op, rop ] |
   \<comment> \<open> P2890 `SHR qwrodregister by CL`   -> ` 0100 100B 1101 001w : 11 101 reg ` \<close>
   Pshrq_r rd  \<Rightarrow>
     let (rex:: u8) = (construct_rex_to_u8  \<comment> \<open> `100B` \<close>
@@ -513,7 +735,10 @@ fun x64_encode :: "instruction \<Rightarrow> x64_bin option" where
     let (op:: u8) = 0xc1 in
     let (rop::u8) = construct_modsib_to_u8 0b11 0b111 (u8_of_ireg rd) in
     let (imm::u8) = ucast n in
-      Some [ rex, op, rop, imm] |
+      if rex = 0x40 then
+        Some [ op, rop, imm ] 
+      else 
+        Some [ rex, op, rop, imm ] |
   \<comment> \<open> P2888 `SAR qwordregister by immediate count` -> ` 0100 100B 1100 000w : 11 111 reg : imm8 ` \<close>
   Psarq_ri rd n \<Rightarrow>
     let (rex:: u8) = (construct_rex_to_u8  \<comment> \<open> `100B` \<close>
@@ -525,7 +750,7 @@ fun x64_encode :: "instruction \<Rightarrow> x64_bin option" where
     let (op:: u8) = 0xc1 in
     let (rop::u8) = construct_modsib_to_u8 0b11 0b111 (u8_of_ireg rd) in
     let (imm::u8) = ucast n in
-      Some [ rex, op, rop, imm] |
+      Some [ rex, op, rop, imm ] |
   \<comment> \<open> P2888 `SAR register by CL`     -> ` 0100 000B 1101 001w : 11 111 reg ` \<close>
   Psarl_r rd  \<Rightarrow>
     let (rex:: u8) = (construct_rex_to_u8  \<comment> \<open> `000B` \<close>
@@ -536,7 +761,10 @@ fun x64_encode :: "instruction \<Rightarrow> x64_bin option" where
       ) in
     let (op:: u8) = 0xd3 in
     let (rop::u8) = construct_modsib_to_u8 0b11 0b111 (u8_of_ireg rd) in
-      Some [ rex, op, rop ] |
+      if rex = 0x40 then
+        Some [ op, rop ] 
+      else 
+        Some [ rex, op, rop ] |
   \<comment> \<open> P2888 `SAR qwordregister by CL`     -> ` 0100 100B 1101 001w : 11 111 reg ` \<close>
   Psarq_r rd  \<Rightarrow>
     let (rex:: u8) = (construct_rex_to_u8  \<comment> \<open> `100B` \<close>
@@ -548,7 +776,49 @@ fun x64_encode :: "instruction \<Rightarrow> x64_bin option" where
     let (op:: u8) = 0xd3 in
     let (rop::u8) = construct_modsib_to_u8 0b11 0b111 (u8_of_ireg rd) in
       Some [ rex, op, rop ] |
-
+  \<comment> \<open> P2877 `BSWAP: register `   -> `0000 1111 : 1100 1 reg` \<close>
+  Pbswapl rd  \<Rightarrow>
+    let (rex:: u8) = (construct_rex_to_u8  \<comment> \<open> `000B` \<close>
+      False \<comment> \<open> W \<close>
+      False \<comment> \<open> R \<close>
+      False \<comment> \<open> X \<close>
+      (and (u8_of_ireg rd) 0b1000 \<noteq> 0) \<comment> \<open> B \<close>
+      ) in
+    let (ex:: u8) = 0x0f in
+    let (op:: u8) = bitfield_insert_u8 0 3 0xc8 (u8_of_ireg rd) in
+      if rex = 0x40 then
+        Some [ex, op]
+      else 
+        Some [rex, ex, op] |
+  \<comment> \<open> P2877 `BSWAP: qwordregister `   -> `0100 100B 0000 1111 : 1100 1 qwordreg` \<close>
+  Pbswapq rd  \<Rightarrow>
+    let (rex:: u8) = (construct_rex_to_u8  \<comment> \<open> `100B` \<close>
+      True \<comment> \<open> W \<close>
+      False \<comment> \<open> R \<close>
+      False \<comment> \<open> X \<close>
+      (and (u8_of_ireg rd) 0b1000 \<noteq> 0) \<comment> \<open> B \<close>
+      ) in
+    let (ex:: u8) = 0x0f in
+    let (op:: u8) = bitfield_insert_u8 0 3 0xc8 (u8_of_ireg rd) in
+      Some [rex, ex, op] |
+  \<comment> \<open> P2881 `LEA: Load Effective Address: in qwordregister `  -> `0100 1RXB : 1000 1101 : mod qwordreg r/m` \<close>
+  Pleaq rd a \<Rightarrow>(
+    case a of Addrmode (Some rb) None dis \<Rightarrow>(
+      let (rex:: u8) = (construct_rex_to_u8  \<comment> \<open> `100B` \<close>
+        True \<comment> \<open> W \<close>
+        (and (u8_of_ireg rd) 0b1000 \<noteq> 0) \<comment> \<open> R \<close>
+        False \<comment> \<open> X \<close>
+        (and (u8_of_ireg rb) 0b1000 \<noteq> 0) \<comment> \<open> B \<close>
+        ) in
+      let (op:: u8) = 0x8d in
+        if dis \<le> 127 \<or> dis \<ge> -128  then   \<comment> \<open> displacement8 : mod 01 \<close>
+          let (dis::u8) = scast dis in
+          let (rop::u8) = construct_modsib_to_u8 0b01 (u8_of_ireg rd) (u8_of_ireg rb) in
+            Some ([ rex, op, rop, dis ])
+        else  \<comment> \<open> displacement32 : mod 10 \<close>
+          let (rop::u8) = construct_modsib_to_u8 0b10 (u8_of_ireg rd) (u8_of_ireg rb) in
+              Some ([ rex, op, rop ] @ (u8_list_of_u32 dis)))
+      | _ \<Rightarrow> None)|
   \<comment> \<open> P2886 `RDTSC – Read Time-Stamp Counter`   -> ` 0000 1111 0011 0001 ` \<close>
   Prdtsc \<Rightarrow>
     let (opes::u8) = 0x0f in
@@ -562,14 +832,13 @@ fun x64_encode :: "instruction \<Rightarrow> x64_bin option" where
       False \<comment> \<open> X \<close>
       (and (u8_of_ireg r1) 0b1000 \<noteq> 0) \<comment> \<open> B \<close>
       ) in
-    let (op::u8) = or 0x50 (and (u8_of_ireg r1) 0b111) in
-      if rex = 0 then
+    let (op::u8) = bitfield_insert_u8 0 3 0x50 (u8_of_ireg r1) in
+      if rex = 0x40 then
         Some [op]
       else 
-        let rex = bitfield_insert_u8 4 4 rex 0x4 in 
-          Some [rex, op] |
+        Some [rex, op] |
   \<comment> \<open> P2885 `PUSH: memory64`   -> ` 0100 W00BS : 1111 1111 : 11 110 reg64 ` \<close>
-  \<comment> \<open> P2885 `PUSH: imm32`   -> ` 0110 1000 : imm32 `(ucast (and n 0xff)),(ucast (n >> 8)),(ucast (n >> 16)),(ucast (n >> 24)) \<close>
+  \<comment> \<open> P2885 `PUSH: imm32`   -> ` 0110 1000 : imm32 ` \<close>
   Ppushl_i n \<Rightarrow>
     let (rex::u8) = (construct_rex_to_u8    \<comment> \<open> `100B` \<close>
       True  \<comment> \<open> W ; Solana may made mistake here, but it won't bring mistakes \<close> 
@@ -579,6 +848,22 @@ fun x64_encode :: "instruction \<Rightarrow> x64_bin option" where
       ) in
     let (op::u8) = 0x68 in
       Some ([rex,op] @ (u8_list_of_u32 n)) |
+  \<comment> \<open> P2885 `PUSH: memory64`   -> `0100 W00BS : 1111 1111 : mod 110 r/m ` \<close>
+  Ppushq_m a M64 \<Rightarrow>(
+    case a of Addrmode (Some rb) (Some (ri,scale)) dis \<Rightarrow>(
+      if scale > 3 then None
+      else 
+        let (rex::u8) = (construct_rex_to_u8    \<comment> \<open> `100B` \<close>
+        True \<comment> \<open> W \<close>
+        False \<comment> \<open> R \<close>
+        (and (u8_of_ireg ri) 0b1000 \<noteq> 0) \<comment> \<open> X \<close>
+        (and (u8_of_ireg rb) 0b1000 \<noteq> 0) \<comment> \<open> B \<close>
+        ) in
+      let (op::u8) = 0xff in 
+      let (rop::u8) = construct_modsib_to_u8 0b10 0b110 0b100 in
+      let (sib::u8) = construct_modsib_to_u8 scale (u8_of_ireg ri) (u8_of_ireg rb) in
+         Some ([rex, op, rop, sib] @ (u8_list_of_u32 dis)))
+    | _ \<Rightarrow> None)|
   \<comment> \<open> P2885 `POP: qwordregister (alternate encoding)`   -> ` 0100 W00B : 0101 1 reg64 ` \<close>
   Ppopl rd \<Rightarrow>
     let (rex::u8) = (construct_rex_to_u8    \<comment> \<open> `000B` \<close>
@@ -587,12 +872,120 @@ fun x64_encode :: "instruction \<Rightarrow> x64_bin option" where
       False \<comment> \<open> X \<close>
       (and (u8_of_ireg rd) 0b1000 \<noteq> 0) \<comment> \<open> B \<close>
       ) in
-    let (op::u8) = or 0x58 (and (u8_of_ireg rd) 0b111) in
-      if rex = 0 then
+    let (op::u8) = bitfield_insert_u8 0 3 0x58 (u8_of_ireg rd) in
+      if rex = 0x40 then
         Some [op]
       else 
-        let rex = bitfield_insert_u8 4 4 rex 0x4 in 
-          Some [rex, op] |
+        Some [rex, op] |
+  \<comment> \<open> P2892 `TEST: register1 and register2`   -> ` 0100 0R0B 1000 010w : 11 reg1 reg2` \<close>
+  Ptestl_rr rd r1 \<Rightarrow>
+    let (rex:: u8) = (construct_rex_to_u8  \<comment> \<open> `0R0B` \<close>
+      False \<comment> \<open> W \<close>
+      (and (u8_of_ireg r1) 0b1000 \<noteq> 0) \<comment> \<open> R \<close>
+      False \<comment> \<open> X \<close>
+      (and (u8_of_ireg rd) 0b1000 \<noteq> 0) \<comment> \<open> B \<close>
+      ) in
+    let (op:: u8) = 0x85 in
+    let (rop::u8) = construct_modsib_to_u8 0b11 (u8_of_ireg r1) (u8_of_ireg rd) in
+      if rex = 0x40 then
+        Some [op, rop]
+      else 
+        Some [rex, op, rop]|
+ \<comment> \<open> P2892 `TEST:  qwordregister1 and qwordregister2`   -> ` 0100 1R0B 1000 0101 : 11 qwordreg1 qwordreg2` \<close>
+  Ptestq_rr rd r1 \<Rightarrow>
+    let (rex:: u8) = (construct_rex_to_u8  \<comment> \<open> `1R0B` \<close>
+      True \<comment> \<open> W \<close>
+      (and (u8_of_ireg r1) 0b1000 \<noteq> 0) \<comment> \<open> R \<close>
+      False \<comment> \<open> X \<close>
+      (and (u8_of_ireg rd) 0b1000 \<noteq> 0) \<comment> \<open> B \<close>
+      ) in
+    let (op:: u8) = 0x85 in
+    let (rop::u8) = construct_modsib_to_u8 0b11 (u8_of_ireg r1) (u8_of_ireg rd) in
+      Some [rex, op, rop]|
+  \<comment> \<open> P2892 `TEST: immediate and register`   -> ` 0100 000B 1111 011w : 11 000 reg : imm ` \<close>
+  Ptestl_ri rd n \<Rightarrow>
+    let (rex:: u8) = (construct_rex_to_u8  \<comment> \<open> `000B` \<close>
+      False \<comment> \<open> W \<close>
+      False \<comment> \<open> R \<close>
+      False \<comment> \<open> X \<close>
+      (and (u8_of_ireg rd) 0b1000 \<noteq> 0) \<comment> \<open> B \<close>
+      ) in
+    let (op:: u8) = 0xf7 in
+    let (rop::u8) = construct_modsib_to_u8 0b11 0b000 (u8_of_ireg rd) in
+      if rex = 0x40 then
+        Some ([op, rop] @ (u8_list_of_u32 n))
+      else 
+        Some ([rex, op, rop] @ (u8_list_of_u32 n))|
+  \<comment> \<open> P2892 `TEST: immediate32 and qwordregister `   -> ` 0100 100B 1111 0111 : 11 000 qwordreg : imm32 ` \<close>
+  Ptestq_ri rd n \<Rightarrow>
+    let (rex:: u8) = (construct_rex_to_u8  \<comment> \<open> `0R0B` \<close>
+      True \<comment> \<open> W \<close>
+      False \<comment> \<open> R \<close>
+      False \<comment> \<open> X \<close>
+      (and (u8_of_ireg rd) 0b1000 \<noteq> 0) \<comment> \<open> B \<close>
+      ) in
+    let (op:: u8) = 0xf7 in
+    let (rop::u8) = construct_modsib_to_u8 0b11 0b000 (u8_of_ireg rd) in
+      Some ([rex, op, rop] @ (u8_list_of_u32 n))|
+  \<comment> \<open> P2878 `CMP: register1 with register2`   -> ` 0100 0R0B 0011 100w : 11 reg1 reg2 ` \<close>
+  Pcmpl_rr r1 r2 \<Rightarrow>
+    let (rex:: u8) = (construct_rex_to_u8  \<comment> \<open> `0R0B` \<close>
+      False \<comment> \<open> W \<close>
+      (and (u8_of_ireg r1) 0b1000 \<noteq> 0) \<comment> \<open> R \<close>
+      False \<comment> \<open> X \<close>
+      (and (u8_of_ireg r2) 0b1000 \<noteq> 0) \<comment> \<open> B \<close>
+      ) in
+    let (op:: u8) = 0x39 in
+    let (rop::u8) = construct_modsib_to_u8 0b11 (u8_of_ireg r1) (u8_of_ireg r2) in
+      if rex = 0x40 then
+        Some [op, rop]
+      else 
+        Some [rex, op, rop] |
+  \<comment> \<open> P2878 `CMP: qwordregister1 with qwordregister2`   -> `0100 1R0B 0011 1001 : 11 qwordreg1 qwordreg2` \<close>
+  Pcmpq_rr r1 r2 \<Rightarrow>
+    let (rex:: u8) = (construct_rex_to_u8  \<comment> \<open> `1R0B` \<close>
+      True  \<comment> \<open> W \<close>
+      (and (u8_of_ireg r1) 0b1000 \<noteq> 0) \<comment> \<open> R \<close>
+      False \<comment> \<open> X \<close>
+      (and (u8_of_ireg r2) 0b1000 \<noteq> 0) \<comment> \<open> B \<close>
+      ) in
+    let (op:: u8) = 0x39 in
+    let (rop::u8) = construct_modsib_to_u8 0b11 (u8_of_ireg r1) (u8_of_ireg r2) in
+      Some [rex, op, rop]|
+  \<comment> \<open> P2878 `CMP: immediate with register`   -> `0100 000B 1000 00sw : 11 111 reg : imm` \<close>
+  Pcmpl_ri r1 n \<Rightarrow>
+    let (rex:: u8) = (construct_rex_to_u8  \<comment> \<open> `0R0B` \<close>
+      False \<comment> \<open> W \<close>
+      False \<comment> \<open> R \<close>
+      False \<comment> \<open> X \<close>
+      (and (u8_of_ireg r1) 0b1000 \<noteq> 0) \<comment> \<open> B \<close>
+      ) in
+    let (op:: u8) = 0x81 in
+    let (rop::u8) = construct_modsib_to_u8 0b11 0b111 (u8_of_ireg r1) in
+      if rex = 0x40 then
+        Some ([op, rop] @ (u8_list_of_u32 n))
+      else 
+        Some ([rex, op, rop] @ (u8_list_of_u32 n))|
+  \<comment> \<open> P2878 `CMP: immediate32 with qwordregister`   -> `0100 100B 1000 0001 : 11 111 qwordreg : imm32` \<close>
+  Pcmpq_ri r1 n \<Rightarrow>
+    let (rex:: u8) = (construct_rex_to_u8  \<comment> \<open> `0R0B` \<close>
+      True \<comment> \<open> W \<close>
+      False \<comment> \<open> R \<close>
+      False \<comment> \<open> X \<close>
+      (and (u8_of_ireg r1) 0b1000 \<noteq> 0) \<comment> \<open> B \<close>
+      ) in
+    let (op:: u8) = 0x81 in
+    let (rop::u8) = construct_modsib_to_u8 0b11 0b111 (u8_of_ireg r1) in
+      Some ([rex, op, rop] @ (u8_list_of_u32 n))|
+  \<comment> \<open> P2881 `JMP: direct` -> `1110 1001 : displacement32` \<close>
+  Pjmp d \<Rightarrow>
+    let (op:: u8) = 0xe9 in
+      Some ([op] @ (u8_list_of_u32 (ucast d)))|
+  \<comment> \<open> P2880 `JCC: full displacement` -> `0000 1111 : 1000 tttn : full displacement` \<close>
+  Pjcc t d \<Rightarrow>
+    let (ex:: u8) = 0x0f in
+    let (op:: u8) = bitfield_insert_u8 0 4 0x80 (u8_of_cond t) in
+    Some ([ex, op] @ (u8_list_of_u32 (ucast d))) |
   \<comment> \<open> P2878 `CALL: register indirect`   -> `0100 W00Bw 1111 1111 : 11 010 reg ` \<close>
   Pcall_r r1 \<Rightarrow>
     let (rex::u8) = (construct_rex_to_u8    \<comment> \<open> `000B` \<close>
@@ -603,15 +996,16 @@ fun x64_encode :: "instruction \<Rightarrow> x64_bin option" where
       ) in
       let (op:: u8) = 0xff in
       let (rop::u8) = construct_modsib_to_u8 0b11 0b010 (u8_of_ireg r1) in
-      if rex = 0 then
+      if rex = 0x40 then
         Some [op, rop]
       else 
-        let rex = bitfield_insert_u8 4 4 rex 0x4 in 
-          Some [rex, op, rop] |
+        Some [rex, op, rop] |
   \<comment> \<open> P2878 `CALL: direct`   -> `1110 1000 : displacement32` \<close>
   Pcall_i d  \<Rightarrow>
-    let (op::u8) = 0xe8 in
-      Some [op,(ucast (and d 0xff)),(ucast (d >> 8)),(ucast (d >> 16)),(ucast (d >> 24))]|
+      Some ([0xe8] @ (u8_list_of_u32 d))|
+  \<comment> \<open> P2887 ` RET near`   -> ` 1100 0011` \<close>
+  Pret \<Rightarrow>
+    Some [0xc3]|
   \<comment> \<open> P2884 `NOP – No Operation` -> `1001 0000` \<close>
   Pnop \<Rightarrow> Some [0x90] |
   _ \<Rightarrow> None
