theory/BitsOpMore2.thy
@@ -1,8 +1,7 @@
 theory BitsOpMore2
 imports
   Main
-  rBPFCommType
-  x64Syntax
+  rBPFCommType 
 begin
 
 lemma ucast64_ucast8_and_255_eq [simp]: "ucast (((ucast (and v 255))::u8)) = and (v:: u64) 255"
@@ -27,7 +26,7 @@ word_of_int (uint v_u8)  :: u64
           subgoal for n4 apply (cases n4, simp_all)
             subgoal for n5 apply (cases n5, simp_all)
               subgoal for n6 apply (cases n6, simp_all)
-                subgoal for n6 apply (cases n6, simp_all)
+                subgoal for n7 apply (cases n7, simp_all)
                   done
                 done
               done
@@ -38,12 +37,7 @@ word_of_int (uint v_u8)  :: u64
     done
   done
 
-lemma [simp]: "n \<ge> 8 \<Longrightarrow> \<not>bit (v::u8) n"
-  apply (rule impossible_bit)
-  apply simp
-  done
-
-lemma [simp]: "n \<le> 56 \<Longrightarrow> ((ucast (v::u8) ::u64) << n) >> n = (ucast (v::u8) ::u64)"
+lemma u64_shl_shr_same : "n \<le> 56 \<Longrightarrow> ((ucast (v::u8) ::u64) << n) >> n = (ucast (v::u8) ::u64)"
   apply (simp add: bit_eq_iff)
   apply (auto simp add: bit_simps)
   subgoal for k
@@ -54,7 +48,7 @@ lemma [simp]: "n \<le> 56 \<Longrightarrow> ((ucast (v::u8) ::u64) << n) >> n = 
           subgoal for n4 apply (cases n4, simp_all)
             subgoal for n5 apply (cases n5, simp_all)
               subgoal for n6 apply (cases n6, simp_all)
-                subgoal for n6 apply (cases n6, simp_all)
+                subgoal for n6 apply (cases n6, simp_all add: u8_ge_8_bit_false)
                   done
                 done
               done
@@ -65,35 +59,18 @@ lemma [simp]: "n \<le> 56 \<Longrightarrow> ((ucast (v::u8) ::u64) << n) >> n = 
     done
   done
 
-lemma [simp]: "n+8 \<le> m \<Longrightarrow> ((ucast (v::u8) ::u64) << n) >> m = (0 ::u64)"
+lemma u64_shl_shr_outside: "n+8 \<le> m \<Longrightarrow> ((ucast (v::u8) ::u64) << n) >> m = (0 ::u64)"
   apply (simp add: bit_eq_iff)
-  apply (auto simp add: bit_simps)
+  apply (auto simp add: bit_simps u8_ge_8_bit_false)
   done
 
 lemma [simp]: "(n::nat) \<le> 56 \<Longrightarrow> m \<le> n \<Longrightarrow> k < 64 \<Longrightarrow> n - m \<le> k \<Longrightarrow> k + m - n < 8 \<Longrightarrow> m + k < 64"
   by simp
 
-lemma [simp]: "bit (v::u8) n \<Longrightarrow> n < 8"
-  apply (cases n, simp_all)
-  subgoal for n1 apply (cases n1, simp_all)
-    subgoal for n2 apply (cases n2, simp_all)
-      subgoal for n3 apply (cases n3, simp_all)
-        subgoal for n4 apply (cases n4, simp_all)
-          subgoal for n5 apply (cases n5, simp_all)
-            subgoal for n6 apply (cases n6, simp_all)
-              subgoal for n6 apply (cases n6, simp_all)
-                done
-              done
-            done
-          done
-        done
-      done
-    done
-  done
-
-lemma [simp]: "n \<le> 56 \<Longrightarrow> m \<le> n \<Longrightarrow> ((ucast (v::u8) ::u64) << n) >> m = ((ucast (v::u8) ::u64) << (n-m))"
+lemma u64_shl_shr_same_minus: "n \<le> 56 \<Longrightarrow> m \<le> n \<Longrightarrow> ((ucast (v::u8) ::u64) << n) >> m =
+  ((ucast (v::u8) ::u64) << (n-m))"
   apply (simp add: bit_eq_iff)
-  apply (auto simp add: bit_simps)
+  apply (auto simp add: bit_simps u8_bit_true_ge_8)
   subgoal for k
     by (simp add: add.commute)
   subgoal for k
@@ -102,10 +79,10 @@ lemma [simp]: "n \<le> 56 \<Longrightarrow> m \<le> n \<Longrightarrow> ((ucast 
 
 lemma [simp]: "8 \<le> m \<Longrightarrow> (ucast (v::u8) ::u64) >> m = (0 ::u64)"
   apply (simp add: bit_eq_iff)
-  apply (auto simp add: bit_simps)
+  apply (auto simp add: bit_simps u8_ge_8_bit_false)
   done
 
-lemma [simp]: "8 \<le> n \<Longrightarrow> (and (or ((v::u64) << n) k) 255) = and k 255"
+lemma u64_and_or_255_same: "8 \<le> n \<Longrightarrow> (and (or ((v::u64) << n) k) 255) = and k 255"
   apply (simp add: bit_eq_iff)
   apply (auto simp add: bit_simps)
   subgoal for t apply (cases t, simp_all)
@@ -126,7 +103,7 @@ lemma [simp]: "8 \<le> n \<Longrightarrow> (and (or ((v::u64) << n) k) 255) = an
     done
   done
 
-lemma [simp]: "(ucast (and (ucast (v::u8)) (255::u64)) ::u8) = v"
+lemma u64_ucast_and_ucast_255_same: "(ucast (and (ucast (v::u8)) (255::u64)) ::u8) = v"
   apply (simp only: ucast_eq)
   apply (simp only: uint_word_of_int_eq word_and_def word_of_int_eq_iff)
   apply simp
@@ -139,8 +116,6 @@ lemma [simp]: "(ucast (and (ucast (v::u8)) (255::u64)) ::u8) = v"
           subgoal for n4 apply (cases n4, simp_all)
             subgoal for n5 apply (cases n5, simp_all)
               subgoal for n6 apply (cases n6, simp_all)
-                subgoal for n6 apply (cases n6, simp_all)
-                  done
                 done
               done
             done
@@ -150,111 +125,108 @@ lemma [simp]: "(ucast (and (ucast (v::u8)) (255::u64)) ::u8) = v"
     done
   done
 
-lemma [simp]: "length l = 8 \<Longrightarrow> l = [l ! 0, l ! Suc 0, l ! 2, l ! 3, l ! 4, l ! 5, l ! 6, l ! 7]"
-  apply (cases l, simp_all)
-  subgoal for a0 l apply (cases l, simp_all)
-    subgoal for a1 l apply (cases l, simp_all)
-      subgoal for a2 l apply (cases l, simp_all)
-        subgoal for a3 l apply (cases l, simp_all)
-          subgoal for a4 l apply (cases l, simp_all)
-            subgoal for a5 l apply (cases l, simp_all)
-              subgoal for a6 l apply (cases l, simp_all)
-                done
-              done
-            done
-          done
-        done
-      done
-    done
-  done
+lemma list_consists_8 : "length l = 8 \<Longrightarrow>
+  l = [l ! 0, l ! Suc 0, l ! 2, l ! 3, l ! 4, l ! 5, l ! 6, l ! 7]"
+  by (metis Cons_nth_drop_Suc One_nat_def add_implies_diff append.simps(1) diff_Suc_1'
+      eval_nat_numeral(2) eval_nat_numeral(3) id_take_nth_drop length_0_conv length_tl
+      less_Suc_eq list.sel(3) nat_1_add_1
+      semiring_norm(26) semiring_norm(27) semiring_norm(28) take0)
 
-lemma [simp]: "bit (255::int) n \<Longrightarrow> n < 8"
-  apply (cases n, simp_all)
-  subgoal for n1 apply (cases n1, simp_all)
-    subgoal for n2 apply (cases n2, simp_all)
-      subgoal for n3 apply (cases n3, simp_all)
-        subgoal for n4 apply (cases n4, simp_all)
-          subgoal for n5 apply (cases n5, simp_all)
-            subgoal for n6 apply (cases n6, simp_all)
-              subgoal for n6 apply (cases n6, simp_all)
-                done
-              done
-            done
-          done
-        done
-      done
-    done
-  done
-
-lemma [simp]: "n \<le> 56 \<Longrightarrow> ((ucast ((ucast (and ((v::u64) >> n) 255)) ::u8) ::u64) << n) =
+lemma u64_ucast_ucast_and_shr_255_shl_same: "n \<le> 56 \<Longrightarrow>
+  ((ucast ((ucast (and ((v::u64) >> n) 255)) ::u8) ::u64) << n) =
   ((and ((v::u64) >> n) 255) << n)"
   apply (simp only: ucast_eq)
   apply (simp only: uint_word_of_int_eq word_and_def word_of_int_eq_iff)
   apply simp
   apply (simp add: bit_eq_iff)
   apply (auto simp add: bit_simps)
+  subgoal for n1
+  using bit_power_k_minus_1_le [of 8 "n1-n"] by simp
   done
 
-lemma bit_power_k_minus_1_le: "bit (2^k -1::int) n \<longleftrightarrow> n < k"
-  apply (simp only: bit_iff_odd)
-  by (simp add: even_decr_exp_div_exp_iff' linorder_not_le)
-
-lemma bit_power_k_minus_1_le_56 [simp]: "bit (0xffffffffffffff::int) n \<longleftrightarrow> n < 56"
-  using bit_power_k_minus_1_le [of 56 n] by simp
-
-(*
-lemma [simp]: "(v::u64) =
-    or (and ((v >> 56) << 56) 18374686479671623680)
-     (or (and ((v >> 48) << 48) 71776119061217280)
-       (or (and ((v >> 40) << 40) 280375465082880)
-         (or (and ((v >> 32) << 32) 1095216660480) (or (and ((v >> 24) << 24) 4278190080)
-            (or (and ((v >> 16) << 16) 16711680) (or (and ((v >> 8) << 8) 65280) (and v 255)))))))"
+lemma [simp]: "and (((v::u64) >> 56) << 56) 18374686479671623680 = and v 18374686479671623680"
   apply (simp add: bit_eq_iff)
-  apply (simp add: bit_or_iff)
+  apply (auto simp add: bit_simps)
+  subgoal for n using bit_power_k_add_m_ge [of 56 8 n] by simp
+  subgoal for n using bit_power_k_add_m_ge [of 56 8 n] by simp
+  done
 
-  apply (rule allI)
-  subgoal for n
-    apply (cases "n \<ge> 56", simp_all)
-    subgoal
+lemma [simp]: "and (((v::u64) >> 48) << 48) 71776119061217280 = and v 71776119061217280"
+  apply (simp add: bit_eq_iff)
+  apply (auto simp add: bit_simps)
+  subgoal for n using bit_power_k_add_m_ge [of 48 8 n] by simp
+  subgoal for n using bit_power_k_add_m_ge [of 48 8 n] by simp
+  done
 
+lemma [simp]: "and (((v::u64) >> 40) << 40) 280375465082880 = and v 280375465082880"
+  apply (simp add: bit_eq_iff)
+  apply (auto simp add: bit_simps)
+  subgoal for n using bit_power_k_add_m_ge [of 40 8 n] by simp
+  subgoal for n using bit_power_k_add_m_ge [of 40 8 n] by simp
+  done
 
-lemma [simp]: "(Some v = u64_of_u8_list l) = (l = u8_list_of_u64 v)"
+lemma [simp]: "and (((v::u64) >> 32) << 32) 1095216660480 = and v 1095216660480"
+  apply (simp add: bit_eq_iff)
+  apply (auto simp add: bit_simps)
+  subgoal for n using bit_power_k_add_m_ge [of 32 8 n] by simp
+  subgoal for n using bit_power_k_add_m_ge [of 32 8 n] by simp
+  done
+
+lemma [simp]: "and (((v::u64) >> 24) << 24) 4278190080 = and v 4278190080"
+  apply (simp add: bit_eq_iff)
+  apply (auto simp add: bit_simps)
+  subgoal for n using bit_power_k_add_m_ge [of 24 8 n] by simp
+  subgoal for n using bit_power_k_add_m_ge [of 24 8 n] by simp
+  done
+
+lemma [simp]: "and (((v::u64) >> 16) << 16) 16711680 = and v 16711680"
+  apply (simp add: bit_eq_iff)
+  apply (auto simp add: bit_simps)
+  subgoal for n using bit_power_k_add_m_ge [of 16 8 n] by simp
+  subgoal for n using bit_power_k_add_m_ge [of 16 8 n] by simp
+  done
+
+lemma [simp]: "and (((v::u64) >> 8) << 8) 65280 = and v 65280"
+  apply (simp add: bit_eq_iff)
+  apply (auto simp add: bit_simps)
+  subgoal for n using bit_power_k_add_m_ge [of 8 8 n] by simp
+  subgoal for n using bit_power_k_add_m_ge [of 8 8 n] by simp
+  done
+
+lemma bit_255_not_lt_64 : "n < 64 \<Longrightarrow>
+  \<not> bit (18374686479671623680::int) n \<Longrightarrow> \<not> bit (71776119061217280::int) n \<Longrightarrow>
+  \<not> bit (280375465082880::int) n \<Longrightarrow> \<not> bit (1095216660480::int) n \<Longrightarrow>
+  \<not> bit (4278190080::int) n \<Longrightarrow> \<not> bit (16711680::int) n \<Longrightarrow>
+  \<not> bit (65280::int) n \<Longrightarrow> bit (255::int) n"
+  using bit_power_k_add_m_lt [of n 56 8] apply simp
+  using bit_power_k_add_m_lt [of n 48 8] apply simp
+  using bit_power_k_add_m_lt [of n 40 8] apply simp
+  using bit_power_k_add_m_lt [of n 32 8] apply simp
+  using bit_power_k_add_m_lt [of n 24 8] apply simp
+  using bit_power_k_add_m_lt [of n 16 8] apply simp
+  using bit_power_k_add_m_lt [of n 8  8] apply simp
+  using bit_power_k_add_m_lt [of n 0  8] apply simp
+  apply blast
+  done
+
+lemma u64_of_u8_list_same: "(Some v = u64_of_u8_list l) = (l = u8_list_of_u64 v)"
   apply (unfold u64_of_u8_list_def u8_list_of_u64_def)
   apply (cases "length l \<noteq> 8", simp_all)
   subgoal by fastforce
   subgoal
     apply (rule iffI)
-    subgoal by simp
+    subgoal
+      apply (simp add: u64_shl_shr_same u64_shl_shr_outside
+          u64_shl_shr_same_minus u64_and_or_255_same u64_ucast_and_ucast_255_same)
+        using list_consists_8 by blast
 
     subgoal
       apply (simp add: bit_eq_iff)
       apply (simp add: bit_or_iff)
-
-
+      apply (auto simp add: bit_simps)
+      subgoal for n
+        using bit_255_not_lt_64 by blast
       done
     done
-  sorry *)
-
-(*lemma [simp]: "u8_list_of_u32 v = l \<Longrightarrow> u32_of_u8_list2 l = Some v " 
-  apply (unfold u8_list_of_u32_def u32_of_u8_list2_def,simp)
-  apply (cases l)
-  subgoal by simp
-  subgoal for v1 l1
-    apply (auto)
-    subgoal
-      apply(cases l1)
-      subgoal by simp
-      subgoal for v2 l2
-        apply(cases l2)
-        subgoal by simp
-        subgoal for v3 l3
-          apply(cases l3)
-          subgoal by simp
-          subgoal for v4 l4
-            apply (cases l4)
-             apply (auto)
-            apply(cases v)
-            subgoal for n*)
-
-
+  done
 end
