theory/x64DecodeProof.thy
@@ -2,80 +2,21 @@ theory x64DecodeProof
 imports
   Main
   rBPFCommType
-  x64Assembler x64Disassembler
+  x64Assembler x64Disassembler BitsOpMore BitsOpMore2 BitsOpMore3 BitsOpMore4
+  x64DecodeProofAux
 begin
-
-lemma [simp]: "l @ [a] = l_bin \<Longrightarrow> l_bin!(length l) = a" by fastforce
-lemma [simp]: "l @ [a, b] = l_bin \<Longrightarrow> l_bin!(length l) = a" by fastforce  
-lemma [simp]: "l @ [a, b, c] = l_bin \<Longrightarrow> l_bin!(length l) = a" by fastforce
-lemma [simp]: "l @ [a, b, c, d] = l_bin \<Longrightarrow> l_bin!(length l) = a" by fastforce
-lemma [simp]: "l @ [a, b, c, d, e] = l_bin \<Longrightarrow> l_bin!(length l) = a" by fastforce
-
-lemma [simp]: "l @ [a, b] = l_bin \<Longrightarrow> l_bin!(length l + 1) = b"
-  by (metis One_nat_def nth_Cons_0 nth_Cons_Suc nth_append_length_plus)
-lemma [simp]: "l @ [a, b, c] = l_bin \<Longrightarrow> l_bin!(length l + 1) = b"
-  by (metis One_nat_def nth_Cons_0 nth_Cons_Suc nth_append_length_plus)
-lemma [simp]: "l @ [a, b, c, d] = l_bin \<Longrightarrow> l_bin!(length l + 1) = b"
-  by (metis One_nat_def nth_Cons_0 nth_Cons_Suc nth_append_length_plus)
-lemma [simp]: "l @ [a, b, c, d, e] = l_bin \<Longrightarrow> l_bin!(length l + 1) = b"
-  by (metis One_nat_def nth_Cons_0 nth_Cons_Suc nth_append_length_plus)
-
-lemma [simp]: "l @ [a, b] = l_bin \<Longrightarrow> l_bin!(Suc (length l)) = b"
-  by (metis One_nat_def add_diff_cancel_right' not_add_less2 nth_Cons_0 nth_Cons_Suc nth_append plus_1_eq_Suc)
-lemma [simp]: "l @ [a, b, c] = l_bin \<Longrightarrow> l_bin!(Suc (length l)) = b"
-  by (metis One_nat_def add_diff_cancel_right' not_add_less2 nth_Cons_0 nth_Cons_Suc nth_append plus_1_eq_Suc)
-lemma [simp]: "l @ [a, b, c, d] = l_bin \<Longrightarrow> l_bin!(Suc (length l)) = b"
-  by (metis One_nat_def add_diff_cancel_right' not_add_less2 nth_Cons_0 nth_Cons_Suc nth_append plus_1_eq_Suc)
-lemma [simp]: "l @ [a, b, c, d, e] = l_bin \<Longrightarrow> l_bin!(Suc (length l)) = b"
-  by (metis One_nat_def add_diff_cancel_right' not_add_less2 nth_Cons_0 nth_Cons_Suc nth_append plus_1_eq_Suc)
-
-lemma [simp]: "l @ [a, b, c] = l_bin \<Longrightarrow> l_bin!(length l + 2) = c"
-  by (metis One_nat_def Suc_1 nth_Cons_0 nth_Cons_Suc nth_append_length_plus)
-lemma [simp]: "l @ [a, b, c, d] = l_bin \<Longrightarrow> l_bin!(length l + 2) = c"
-  by (metis One_nat_def Suc_1 nth_Cons_0 nth_Cons_Suc nth_append_length_plus)
-lemma [simp]: "l @ [a, b, c, d, e] = l_bin \<Longrightarrow> l_bin!(length l + 2) = c"
-  by (metis One_nat_def Suc_1 nth_Cons_0 nth_Cons_Suc nth_append_length_plus)
-
-
-lemma [simp]: "l @ [a, b, c] = l_bin \<Longrightarrow> l_bin!(Suc (Suc (length l))) = c"
-  by (metis Cons_eq_appendI One_nat_def add_Suc_right append_Nil length_append list.size(3) list.size(4) nth_append_length nth_append_length_plus plus_1_eq_Suc)
-lemma [simp]: "l @ [a, b, c, d] = l_bin \<Longrightarrow> l_bin!(Suc (Suc (length l))) = c"
-  by (metis Cons_eq_appendI One_nat_def add_Suc_right append_Nil length_append list.size(3) list.size(4) nth_append_length nth_append_length_plus plus_1_eq_Suc)
-lemma [simp]: "l @ [a, b, c, d, e] = l_bin \<Longrightarrow> l_bin!(Suc (Suc (length l))) = c"
-  by (metis Cons_eq_appendI One_nat_def add_Suc_right append_Nil length_append list.size(3) list.size(4) nth_append_length nth_append_length_plus plus_1_eq_Suc)
-
-lemma [simp]: "l @ [a, b, c, d] = l_bin \<Longrightarrow> l_bin!(length l + 3) = d"
-  by force
-lemma [simp]: "l @ [a, b, c, d, e] = l_bin \<Longrightarrow> l_bin!(length l + 3) = d"
-  by force
-
-
-lemma [simp]: "l @ [a, b, c, d] = l_bin \<Longrightarrow> l_bin!(Suc (Suc (Suc (length l)))) = d"
-  by (metis One_nat_def Suc3_eq_add_3 add_diff_cancel_right' last.simps last_conv_nth length_Cons list.discI list.size(3) not_add_less2 nth_append)
-lemma [simp]: "l @ [a, b, c, d, e] = l_bin \<Longrightarrow> l_bin!(Suc (Suc (Suc (length l)))) = d"
-  by (metis Suc3_eq_add_3 add.commute nth_Cons_0 nth_Cons_Suc nth_append_length_plus numeral_3_eq_3)
-
-lemma [simp]: "l @ [a, b, c, d, e] = l_bin \<Longrightarrow> l_bin!(length l + 4) = e"
-  by force
-
-lemma [simp]: "l @ [a, b, c, d, e] = l_bin \<Longrightarrow> l_bin!(Suc (Suc (Suc (Suc (length l))))) = e"
-  by (metis Nil_is_append_conv One_nat_def Suc_1 add_2_eq_Suc' add_Suc_right diff_Suc_1' last.simps last_appendR last_conv_nth length_Cons length_append list.discI list.size(3))
-
-lemma [simp]: "l @ [a] = l_bin \<Longrightarrow> length l_bin - length l = 1" by fastforce
-lemma [simp]: "l @ [a, b] = l_bin \<Longrightarrow> length l_bin - length l = 2" by fastforce  
-lemma [simp]: "l @ [a, b, c] = l_bin \<Longrightarrow> length l_bin - length l = 3" by fastforce
-lemma [simp]: "l @ [a, b, c, d] = l_bin \<Longrightarrow> length l_bin - length l = 4" by fastforce
-lemma [simp]: "l @ [a, b, c, d, e] = l_bin \<Longrightarrow> length l_bin - length l = 5" by fastforce
-
+(* It may take more than one hour to run this proof *)
+declare if_split_asm [split]
 
 lemma x64_encode_decode_consistency:
-  "list_in_list l_bin pc l \<Longrightarrow> Some l_bin = x64_encode ins \<Longrightarrow> x64_decode pc l = Some (length l_bin, ins)"
+  "list_in_list l_bin pc l \<Longrightarrow> Some l_bin = x64_encode ins \<Longrightarrow>
+    x64_decode pc l = Some (length l_bin, ins)"
   apply (cases ins; simp_all)
 
   subgoal for dst src
   \<comment> \<open> Pmovl_rr \<close> 
     apply (unfold Let_def)
-    apply (cases "construct_rex_to_u8 False (and (u8_of_ireg src) 8 \<noteq> 0) False (and (u8_of_ireg dst) 8 \<noteq> 0) = 0"; simp_all add: construct_rex_to_u8_def construct_modsib_to_u8_def; erule conjE)
+    apply (cases "construct_rex_to_u8 False (and (u8_of_ireg src) 8 \<noteq> 0) False (and (u8_of_ireg dst) 8 \<noteq> 0) = 64"; simp_all add: construct_rex_to_u8_def construct_modsib_to_u8_def; erule conjE)
     subgoal by (cases src; cases dst; auto simp add: x64_decode_def bitfield_insert_u8_def Let_def ireg_of_u8_def)
     subgoal by (cases src; cases dst; auto simp add: x64_decode_def bitfield_insert_u8_def Let_def ireg_of_u8_def)
     done
@@ -86,37 +27,1100 @@ lemma x64_encode_decode_consistency:
     subgoal by (cases src; cases dst; auto simp add: x64_decode_def bitfield_insert_u8_def Let_def ireg_of_u8_def)
     done
 
-  subgoal for dst src sorry
+  subgoal for dst imm
+  \<comment> \<open> Pmovl_ri  \<close>
+    apply (unfold Let_def)
+    apply (cases "construct_rex_to_u8 False False False (and (u8_of_ireg dst) 8 \<noteq> 0) = 64";
+        simp_all add:construct_rex_to_u8_def construct_modsib_to_u8_def; erule conjE)
+    subgoal \<comment> \<open> rex = 0x40  \<close>
+      using list_in_list_u8_list_of_u32_simp_sym [of imm "(Suc (Suc pc))" l]
+      using length_u8_list_of_u32_eq_4
+      apply (cases dst; auto simp add: x64_decode_def bitfield_insert_u8_def Let_def
+          ireg_of_u8_def Suc3_eq_add_3 add.commute)
+      done
 
-  subgoal for dst src sorry
+    subgoal \<comment> \<open> rex <> 0x40  \<close>
+      using list_in_list_u8_list_of_u32_simp_sym [of imm "(pc+3)" l]
+      using length_u8_list_of_u32_eq_4
+      apply (cases dst; auto simp add: x64_decode_def bitfield_insert_u8_def Let_def
+          ireg_of_u8_def Suc3_eq_add_3 add.commute)
+      done
+    done
 
-  subgoal for src dst chunk
-  \<comment> \<open> Pmov_rm \<close> 
-    apply (cases dst, simp)
-    subgoal for rd rs ro
-      apply (cases rd, simp_all)
-      subgoal for rd1
-        apply (cases rs, simp_all)
-        apply (cases "rd1 = ireg.R11 \<and> ro = 0", simp_all add: Let_def)
-        apply (unfold Let_def construct_rex_to_u8_def construct_modsib_to_u8_def)
-        apply (cases chunk; cases src; auto simp add: x64_decode_def bitfield_insert_u8_def Let_def ireg_of_u8_def)
+  subgoal for dst imm
+ \<comment> \<open> Pmovq_ri\<close>
+    apply (unfold Let_def construct_rex_to_u8_def construct_modsib_to_u8_def)
+    using list_in_list_u8_list_of_u64_simp_sym [of imm "(Suc (Suc pc))" l]
+    using length_u8_list_of_u64_eq_8
+    apply (cases dst; simp_all add: bitfield_insert_u8_def x64_decode_def ireg_of_u8_def Suc3_eq_add_3 add.commute)
+    done
+
+  subgoal for dst addr chunk
+  \<comment> \<open> Pmov_rm \<close>
+    apply (cases addr, simp)
+    subgoal for base index2 ofs
+      apply (cases base; simp)
+      subgoal for base_reg
+        apply (cases index2; simp add: Let_def)
+        subgoal \<comment> \<open> ofs < u8 /\ index2 = None  /\ not rex \<close>
+          apply (cases chunk; simp)
+          apply (unfold construct_rex_to_u8_def construct_modsib_to_u8_def
+              bitfield_insert_u8_def Let_def)
+          using scast_u32_scast_u8_eq
+          apply (cases dst; simp; cases base_reg; simp add: x64_decode_def Let_def ireg_of_u8_def
+                bitfield_insert_u8_def)
+          done
+
+        subgoal \<comment> \<open> ofs < u8 /\ index2 = None  /\ has rex \<close>
+
+          using scast_u32_scast_u8_eq
+          apply (cases chunk; simp add: construct_rex_to_u8_def construct_modsib_to_u8_def
+            bitfield_insert_u8_def Let_def)
+          subgoal \<comment> \<open> index2 = None  /\ has rex  /\ M32 \<close>
+            apply (cases dst; simp; cases base_reg; simp add: x64_decode_def Let_def ireg_of_u8_def
+                  bitfield_insert_u8_def  Suc3_eq_add_3 add.commute)
+            done
+          subgoal \<comment> \<open> index2 = None  /\ has rex  /\ M64 \<close>
+            apply (cases dst; simp; cases base_reg; simp add: x64_decode_def Let_def ireg_of_u8_def
+                  bitfield_insert_u8_def  Suc3_eq_add_3 add.commute)
+            done
+          done 
+
+        subgoal \<comment> \<open> ofs > u8 /\ index2 = None  /\ not rex \<close>
+          apply (cases chunk; simp; erule conjE)
+          apply (unfold construct_rex_to_u8_def construct_modsib_to_u8_def
+              bitfield_insert_u8_def Let_def)
+
+          using list_in_list_u8_list_of_u32_simp_sym [of ofs "(Suc (Suc pc))" l]
+          using length_u8_list_of_u32_eq_4
+
+          apply (cases dst; simp; cases base_reg; simp add: x64_decode_def Let_def ireg_of_u8_def
+                    bitfield_insert_u8_def Suc3_eq_add_3 add.commute)
+          done 
+
+        subgoal \<comment> \<open> ofs > u8 /\ index2 = None  /\ has rex \<close>
+          apply (cases chunk; simp; erule conjE; erule conjE; erule conjE)
+          apply (unfold construct_rex_to_u8_def construct_modsib_to_u8_def
+              bitfield_insert_u8_def Let_def)
+          subgoal  \<comment> \<open> M32 \<close>
+            using list_in_list_u8_list_of_u32_simp_sym [of ofs "(Suc (Suc (Suc pc)))" l]
+            using length_u8_list_of_u32_eq_4
+            apply (cases dst; simp; cases base_reg; simp add: x64_decode_def Let_def ireg_of_u8_def
+                    bitfield_insert_u8_def Suc3_eq_add_3 Suc4_eq_add_4 add.commute)
+            done
+          subgoal  \<comment> \<open> M64 \<close>
+            using list_in_list_u8_list_of_u32_simp_sym [of ofs "(Suc (Suc (Suc pc)))" l]
+            using length_u8_list_of_u32_eq_4
+            apply (cases dst; simp; cases base_reg; simp add: x64_decode_def Let_def ireg_of_u8_def
+                    bitfield_insert_u8_def Suc3_eq_add_3 Suc4_eq_add_4 add.commute)
+            done
+          done
+
+        subgoal for index22\<comment> \<open> index2 = Some \<close>
+          apply(cases chunk; cases index22;simp_all)
+          subgoal for index_reg scale
+            apply (erule conjE; erule conjE; erule conjE; erule conjE)
+            using list_in_list_u8_list_of_u32_simp_sym [of "ofs" " (Suc (Suc (Suc (Suc pc))))" l]
+            using length_u8_list_of_u32_eq_4
+            using construct_modsib_to_u8_imply_index_reg [of " (and (u8_of_ireg dst) 8 \<noteq> 0)" index_reg base_reg "l ! pc" scale "l ! (Suc (Suc (Suc pc)))"]
+            using construct_modsib_to_u8_imply_base_reg  [of " (and (u8_of_ireg dst) 8 \<noteq> 0)" index_reg base_reg "l ! pc" scale "l ! (Suc (Suc (Suc pc)))"]
+            using construct_modsib_to_u8_imply_scale [of scale index_reg base_reg "l !  Suc (Suc (Suc pc))"]
+              apply (cases dst; simp add: construct_rex_to_u8_def  construct_modsib_to_u8_def)
+              subgoal by (cases base_reg; simp; cases index_reg; simp add: x64_decode_def
+                     bitfield_insert_u8_def Let_def ireg_of_u8_def
+                    add.commute Suc3_eq_add_3 Suc4_eq_add_4) 
+              subgoal by (cases base_reg; simp; cases index_reg; simp add: x64_decode_def
+                     bitfield_insert_u8_def Let_def ireg_of_u8_def
+                    add.commute Suc3_eq_add_3 Suc4_eq_add_4) 
+              subgoal by (cases base_reg; simp; cases index_reg; simp add: x64_decode_def
+                     bitfield_insert_u8_def Let_def ireg_of_u8_def
+                    add.commute Suc3_eq_add_3 Suc4_eq_add_4) 
+              subgoal by (cases base_reg; simp; cases index_reg; simp add: x64_decode_def
+                     bitfield_insert_u8_def Let_def ireg_of_u8_def
+                    add.commute Suc3_eq_add_3 Suc4_eq_add_4) 
+              subgoal by (cases base_reg; simp; cases index_reg; simp add: x64_decode_def
+                     bitfield_insert_u8_def Let_def ireg_of_u8_def
+                    add.commute Suc3_eq_add_3 Suc4_eq_add_4) 
+              subgoal by (cases base_reg; simp; cases index_reg; simp add: x64_decode_def
+                     bitfield_insert_u8_def Let_def ireg_of_u8_def
+                    add.commute Suc3_eq_add_3 Suc4_eq_add_4) 
+              subgoal by (cases base_reg; simp; cases index_reg; simp add: x64_decode_def
+                     bitfield_insert_u8_def Let_def ireg_of_u8_def
+                    add.commute Suc3_eq_add_3 Suc4_eq_add_4) 
+              subgoal by (cases base_reg; simp; cases index_reg; simp add: x64_decode_def
+                     bitfield_insert_u8_def Let_def ireg_of_u8_def
+                    add.commute Suc3_eq_add_3 Suc4_eq_add_4) 
+              subgoal by (cases base_reg; simp; cases index_reg; simp add: x64_decode_def
+                     bitfield_insert_u8_def Let_def ireg_of_u8_def
+                    add.commute Suc3_eq_add_3 Suc4_eq_add_4) 
+              subgoal by (cases base_reg; simp; cases index_reg; simp add: x64_decode_def
+                     bitfield_insert_u8_def Let_def ireg_of_u8_def
+                    add.commute Suc3_eq_add_3 Suc4_eq_add_4) 
+              subgoal by (cases base_reg; simp; cases index_reg; simp add: x64_decode_def
+                     bitfield_insert_u8_def Let_def ireg_of_u8_def
+                    add.commute Suc3_eq_add_3 Suc4_eq_add_4) 
+              subgoal by (cases base_reg; simp; cases index_reg; simp add: x64_decode_def
+                     bitfield_insert_u8_def Let_def ireg_of_u8_def
+                    add.commute Suc3_eq_add_3 Suc4_eq_add_4) 
+              subgoal by (cases base_reg; simp; cases index_reg; simp add: x64_decode_def
+                     bitfield_insert_u8_def Let_def ireg_of_u8_def
+                    add.commute Suc3_eq_add_3 Suc4_eq_add_4) 
+              subgoal by (cases base_reg; simp; cases index_reg; simp add: x64_decode_def
+                     bitfield_insert_u8_def Let_def ireg_of_u8_def
+                    add.commute Suc3_eq_add_3 Suc4_eq_add_4) 
+              subgoal by (cases base_reg; simp; cases index_reg; simp add: x64_decode_def
+                     bitfield_insert_u8_def Let_def ireg_of_u8_def
+                    add.commute Suc3_eq_add_3 Suc4_eq_add_4) 
+              subgoal by (cases base_reg; simp; cases index_reg; simp add: x64_decode_def
+                     bitfield_insert_u8_def Let_def ireg_of_u8_def
+                    add.commute Suc3_eq_add_3 Suc4_eq_add_4) 
+            done
+          done
         done
       done
     done
 
- \<comment> \<open> 
-    apply (cases src)
-    subgoal
-      apply (cases dst)
-      subgoal
-        apply (auto simp add: bitfield_insert_u8_def Let_def u8_of_bool_def)
-        apply (unfold x64_decode_def Let_def)
-        apply simp
-        value "unsigned_bitfield_extract_u8 4 4 (8)"
 
-        apply (auto simp add: bitfield_insert_u8_def Let_def ireg_of_u8_def)
+  subgoal for addr r1 chunk
+    \<comment> \<open> Pmov_mr \<close> 
+      \<comment> \<open> Pmov_rm \<close>
+    apply (cases addr ;simp_all)
+    subgoal for base index2 ofs
+      apply (cases base; simp_all)
+      subgoal for base_reg
+        apply (cases index2; simp add: Let_def)
 
+        subgoal \<comment> \<open> ofs < u8 \<and> index2 = None \<and>  not rex \<close>
+        using scast_u32_scast_u8_eq
+          apply (cases chunk; simp_all add:construct_rex_to_u8_def construct_modsib_to_u8_def
+              bitfield_insert_u8_def Let_def)
+          apply (erule conjE; erule conjE)
+          subgoal by(cases r1; simp; cases base_reg; simp add: x64_decode_def Let_def ireg_of_u8_def
+                bitfield_insert_u8_def )
+          subgoal by(cases r1; simp; cases base_reg; simp add: x64_decode_def Let_def ireg_of_u8_def
+                bitfield_insert_u8_def  Suc3_eq_add_3 add.commute)
+          subgoal by(cases r1; simp; cases base_reg; simp add: x64_decode_def Let_def ireg_of_u8_def
+                bitfield_insert_u8_def )
+          done
+
+
+        subgoal \<comment> \<open> ofs < u8 \<and> index2 = None \<and> has rex \<close>
+          using scast_u32_scast_u8_eq
+          apply (cases chunk; simp_all add:construct_rex_to_u8_def construct_modsib_to_u8_def
+              bitfield_insert_u8_def Let_def)
+               apply (erule conjE; erule conjE;erule conjE)
+          subgoal
+            by (cases r1; simp; cases base_reg;simp_all add: x64_decode_def Let_def ireg_of_u8_def
+                  bitfield_insert_u8_def Suc3_eq_add_3 add.commute )
+          subgoal
+            by (cases r1; simp; cases base_reg; simp add: x64_decode_def Let_def ireg_of_u8_def
+                bitfield_insert_u8_def  Suc3_eq_add_3 add.commute)
+          subgoal
+            by (cases r1; simp; cases base_reg; simp add: x64_decode_def Let_def ireg_of_u8_def
+                bitfield_insert_u8_def  Suc3_eq_add_3 add.commute)
+          subgoal
+            by (cases r1; simp; cases base_reg; simp add: x64_decode_def Let_def ireg_of_u8_def
+                bitfield_insert_u8_def  Suc3_eq_add_3 add.commute)
+            done
+
+
+
+        subgoal \<comment> \<open> ofs > u8 /\ index2 = None  /\ not rex \<close>
+          apply (cases chunk; simp; erule conjE)
+          apply (unfold construct_rex_to_u8_def construct_modsib_to_u8_def; erule conjE)
+
+          using list_in_list_u8_list_of_u32_simp_sym [of ofs "(Suc (Suc pc))" l]
+          using length_u8_list_of_u32_eq_4
+
+          apply (cases r1; simp; cases base_reg; simp add: x64_decode_def Let_def ireg_of_u8_def
+                    bitfield_insert_u8_def Suc3_eq_add_3 add.commute)
+          done 
+
+        subgoal \<comment> \<open> ofs > u8 /\ index2 = None  /\ has rex \<close>
+          apply (cases chunk; simp; erule conjE; erule conjE; erule conjE)
+          apply (unfold construct_rex_to_u8_def construct_modsib_to_u8_def
+              bitfield_insert_u8_def Let_def)
+          subgoal  \<comment> \<open> M32 \<close>
+            using list_in_list_u8_list_of_u32_simp_sym [of ofs "(Suc (Suc (Suc pc)))" l]
+            using length_u8_list_of_u32_eq_4
+            apply (cases r1; simp; cases base_reg; simp add: x64_decode_def Let_def ireg_of_u8_def
+                    bitfield_insert_u8_def Suc3_eq_add_3 Suc4_eq_add_4 add.commute)
+            done
+          subgoal  \<comment> \<open> M64 \<close>
+            using list_in_list_u8_list_of_u32_simp_sym [of ofs "(Suc (Suc (Suc pc)))" l]
+            using length_u8_list_of_u32_eq_4
+            apply (cases r1; simp; cases base_reg; simp add: x64_decode_def Let_def ireg_of_u8_def
+                    bitfield_insert_u8_def Suc3_eq_add_3 Suc4_eq_add_4 add.commute)
+            done
+          done
+
+        subgoal for index22\<comment> \<open> index2 = Some \<close>
+          apply(cases chunk; cases index22;simp_all)
+          subgoal for index_reg scale
+            apply (erule conjE; erule conjE; erule conjE; erule conjE)
+            using list_in_list_u8_list_of_u32_simp_sym [of "ofs" " (Suc (Suc (Suc (Suc pc))))" l]
+            using length_u8_list_of_u32_eq_4
+            using construct_modsib_to_u8_imply_index_reg [of " (and (u8_of_ireg r1) 8 \<noteq> 0)" index_reg base_reg "l ! pc" scale "l ! (Suc (Suc (Suc pc)))"]
+            using construct_modsib_to_u8_imply_base_reg  [of " (and (u8_of_ireg r1) 8 \<noteq> 0)" index_reg base_reg "l ! pc" scale "l ! (Suc (Suc (Suc pc)))"]
+            using construct_modsib_to_u8_imply_scale [of scale index_reg base_reg "l !  Suc (Suc (Suc pc))"]
+              apply (cases r1; simp add: construct_rex_to_u8_def  construct_modsib_to_u8_def)
+              subgoal by (cases base_reg; simp; cases index_reg; simp add: x64_decode_def
+                     bitfield_insert_u8_def Let_def ireg_of_u8_def
+                    add.commute Suc3_eq_add_3 Suc4_eq_add_4) 
+              subgoal by (cases base_reg; simp; cases index_reg; simp add: x64_decode_def
+                     bitfield_insert_u8_def Let_def ireg_of_u8_def
+                    add.commute Suc3_eq_add_3 Suc4_eq_add_4) 
+              subgoal by (cases base_reg; simp; cases index_reg; simp add: x64_decode_def
+                     bitfield_insert_u8_def Let_def ireg_of_u8_def
+                    add.commute Suc3_eq_add_3 Suc4_eq_add_4) 
+              subgoal by (cases base_reg; simp; cases index_reg; simp add: x64_decode_def
+                     bitfield_insert_u8_def Let_def ireg_of_u8_def
+                    add.commute Suc3_eq_add_3 Suc4_eq_add_4) 
+              subgoal by (cases base_reg; simp; cases index_reg; simp add: x64_decode_def
+                     bitfield_insert_u8_def Let_def ireg_of_u8_def
+                    add.commute Suc3_eq_add_3 Suc4_eq_add_4) 
+              subgoal by (cases base_reg; simp; cases index_reg; simp add: x64_decode_def
+                     bitfield_insert_u8_def Let_def ireg_of_u8_def
+                    add.commute Suc3_eq_add_3 Suc4_eq_add_4) 
+              subgoal by (cases base_reg; simp; cases index_reg; simp add: x64_decode_def
+                     bitfield_insert_u8_def Let_def ireg_of_u8_def
+                    add.commute Suc3_eq_add_3 Suc4_eq_add_4) 
+              subgoal by (cases base_reg; simp; cases index_reg; simp add: x64_decode_def
+                     bitfield_insert_u8_def Let_def ireg_of_u8_def
+                    add.commute Suc3_eq_add_3 Suc4_eq_add_4) 
+              subgoal by (cases base_reg; simp; cases index_reg; simp add: x64_decode_def
+                     bitfield_insert_u8_def Let_def ireg_of_u8_def
+                    add.commute Suc3_eq_add_3 Suc4_eq_add_4) 
+              subgoal by (cases base_reg; simp; cases index_reg; simp add: x64_decode_def
+                     bitfield_insert_u8_def Let_def ireg_of_u8_def
+                    add.commute Suc3_eq_add_3 Suc4_eq_add_4) 
+              subgoal by (cases base_reg; simp; cases index_reg; simp add: x64_decode_def
+                     bitfield_insert_u8_def Let_def ireg_of_u8_def
+                    add.commute Suc3_eq_add_3 Suc4_eq_add_4) 
+              subgoal by (cases base_reg; simp; cases index_reg; simp add: x64_decode_def
+                     bitfield_insert_u8_def Let_def ireg_of_u8_def
+                    add.commute Suc3_eq_add_3 Suc4_eq_add_4) 
+              subgoal by (cases base_reg; simp; cases index_reg; simp add: x64_decode_def
+                     bitfield_insert_u8_def Let_def ireg_of_u8_def
+                    add.commute Suc3_eq_add_3 Suc4_eq_add_4) 
+              subgoal by (cases base_reg; simp; cases index_reg; simp add: x64_decode_def
+                     bitfield_insert_u8_def Let_def ireg_of_u8_def
+                    add.commute Suc3_eq_add_3 Suc4_eq_add_4) 
+              subgoal by (cases base_reg; simp; cases index_reg; simp add: x64_decode_def
+                     bitfield_insert_u8_def Let_def ireg_of_u8_def
+                    add.commute Suc3_eq_add_3 Suc4_eq_add_4) 
+              subgoal by (cases base_reg; simp; cases index_reg; simp add: x64_decode_def
+                     bitfield_insert_u8_def Let_def ireg_of_u8_def
+                    add.commute Suc3_eq_add_3 Suc4_eq_add_4) 
+            done
+          done
+        done
+      done
+    done
+
+  subgoal for addr imm chunk
+    \<comment> \<open> Pmov_mi \<close> 
+    apply(cases chunk, simp_all)
+    apply (cases addr, simp)
+    subgoal for base index2 ofs
+      apply (cases base, simp_all)
+      subgoal for base_reg
+        apply (cases index2; simp add: Let_def; erule conjE; erule conjE; erule conjE; erule conjE)
+        subgoal
+          apply (auto simp add: construct_rex_to_u8_def construct_modsib_to_u8_def)
+          subgoal
+            using list_in_list_u8_list_of_u32_simp_sym [of imm "(Suc (Suc (Suc (Suc pc))))" l]
+            using length_u8_list_of_u32_eq_4 
+            using scast_u32_scast_u8_eq
+              by (cases base_reg;auto simp add: x64_decode_def Let_def ireg_of_u8_def
+                bitfield_insert_u8_def Suc3_eq_add_3 Suc4_eq_add_4 add.commute)
+            subgoal
+            using list_in_list_u8_list_of_u32_simp_sym [of imm "(Suc (Suc (Suc (Suc pc))))" l]
+            using length_u8_list_of_u32_eq_4 
+            using scast_u32_scast_u8_eq
+            by (cases base_reg;auto simp add: x64_decode_def Let_def ireg_of_u8_def
+                bitfield_insert_u8_def Suc3_eq_add_3 Suc4_eq_add_4 add.commute)
+          done
+        subgoal
+          apply (simp add: list_in_list_concat length_u8_list_of_u32_eq_4)
+          using list_in_list_u8_list_of_u32_simp_sym [of "ofs" "(Suc (Suc (Suc pc)))" l]
+          using list_in_list_u8_list_of_u32_simp_sym [of imm "(7 + pc)" l]
+          apply (cases base_reg; simp add: x64_decode_def  construct_rex_to_u8_def bitfield_insert_u8_def 
+              Let_def construct_modsib_to_u8_def ireg_of_u8_def Suc3_eq_add_3 Suc4_eq_add_4 add.commute)
+          done
+        done
+      done
+    done
+
+  subgoal for test dst src
+    \<comment> \<open> Pcmovl \<close>
+    apply (unfold Let_def construct_rex_to_u8_def construct_modsib_to_u8_def)
+    subgoal by (cases test; simp; cases dst; simp; cases src, simp_all add: x64_decode_def bitfield_insert_u8_def
+          Let_def ireg_of_u8_def cond_of_u8_def  Suc3_eq_add_3 add.commute)
+    done
+
+
+  subgoal for test dst src
+    \<comment> \<open> Pcmovq \<close>
+    apply (unfold Let_def construct_rex_to_u8_def construct_modsib_to_u8_def)
+    subgoal by (cases test; simp; cases dst; simp; cases src, simp_all add: x64_decode_def bitfield_insert_u8_def
+          Let_def ireg_of_u8_def cond_of_u8_def  Suc3_eq_add_3 add.commute)
+    done
+
+
+  subgoal for dst src
+    \<comment> \<open> Pxchgq_rr \<close>
+    apply (unfold Let_def construct_rex_to_u8_def construct_modsib_to_u8_def)
     subgoal by (cases src; cases dst; auto simp add: x64_decode_def bitfield_insert_u8_def Let_def ireg_of_u8_def)
- \<close> 
+    done
+
+  subgoal for dst addr chunk
+    \<comment> \<open> Pxchgq_rm \<close> 
+    apply (cases chunk; simp_all)
+    apply (cases addr, simp)
+    subgoal for base index2 ofs
+      apply (cases base;simp)
+      subgoal for base_reg
+        apply (cases index2; simp add: Let_def)
+        subgoal for index22
+          apply (cases index22, simp_all)
+          subgoal for index_reg scale
+            apply (erule conjE;erule conjE;erule conjE;erule conjE)
+
+            using list_in_list_u8_list_of_u32_simp_sym [of ofs "(Suc (Suc (Suc (Suc pc))))" l]
+            using length_u8_list_of_u32_eq_4
+            using construct_modsib_to_u8_imply_index_reg [of "(and (u8_of_ireg dst) 8 \<noteq> 0)" index_reg base_reg "l ! pc" scale "l ! Suc (Suc (Suc pc))"]
+            using construct_modsib_to_u8_imply_base_reg [of "(and (u8_of_ireg dst) 8 \<noteq> 0)" index_reg base_reg "l ! pc" scale "l ! Suc (Suc (Suc pc))"]
+            using construct_modsib_to_u8_imply_scale [of scale index_reg base_reg "l ! Suc (Suc (Suc pc))"]
+                       (*      apply (simp_all add: construct_rex_to_u8_def construct_modsib_to_u8_def)*)
+              apply (cases dst; simp add: construct_rex_to_u8_def  construct_modsib_to_u8_def)
+
+              subgoal by (cases index_reg; simp; cases base_reg; simp add: x64_decode_def bitfield_insert_u8_def Let_def ireg_of_u8_def
+                      Suc3_eq_add_3 Suc4_eq_add_4 add.commute)
+
+              subgoal by (cases index_reg; simp; cases base_reg; simp add: x64_decode_def bitfield_insert_u8_def Let_def ireg_of_u8_def
+                      Suc3_eq_add_3 Suc4_eq_add_4 add.commute)
+
+              subgoal by (cases index_reg; simp; cases base_reg; simp add: x64_decode_def bitfield_insert_u8_def Let_def ireg_of_u8_def
+                      Suc3_eq_add_3 Suc4_eq_add_4 add.commute)
+
+              subgoal by (cases index_reg; simp; cases base_reg; simp add: x64_decode_def bitfield_insert_u8_def Let_def ireg_of_u8_def
+                      Suc3_eq_add_3 Suc4_eq_add_4 add.commute)
+
+              subgoal by (cases index_reg; simp; cases base_reg; simp add: x64_decode_def bitfield_insert_u8_def Let_def ireg_of_u8_def
+                      Suc3_eq_add_3 Suc4_eq_add_4 add.commute)
+
+              subgoal by (cases index_reg; simp; cases base_reg; simp add: x64_decode_def bitfield_insert_u8_def Let_def ireg_of_u8_def
+                      Suc3_eq_add_3 Suc4_eq_add_4 add.commute)
+
+              subgoal by (cases index_reg; simp; cases base_reg; simp add: x64_decode_def bitfield_insert_u8_def Let_def ireg_of_u8_def
+                      Suc3_eq_add_3 Suc4_eq_add_4 add.commute)
+
+              subgoal by (cases index_reg; simp; cases base_reg; simp add: x64_decode_def bitfield_insert_u8_def Let_def ireg_of_u8_def
+                      Suc3_eq_add_3 Suc4_eq_add_4 add.commute)
+
+              subgoal by (cases index_reg; simp; cases base_reg; simp add: x64_decode_def bitfield_insert_u8_def Let_def ireg_of_u8_def
+                      Suc3_eq_add_3 Suc4_eq_add_4 add.commute)
+
+              subgoal by (cases index_reg; simp; cases base_reg; simp add: x64_decode_def bitfield_insert_u8_def Let_def ireg_of_u8_def
+                      Suc3_eq_add_3 Suc4_eq_add_4 add.commute)
+
+              subgoal by (cases index_reg; simp; cases base_reg; simp add: x64_decode_def bitfield_insert_u8_def Let_def ireg_of_u8_def
+                      Suc3_eq_add_3 Suc4_eq_add_4 add.commute)
+
+              subgoal by (cases index_reg; simp; cases base_reg; simp add: x64_decode_def bitfield_insert_u8_def Let_def ireg_of_u8_def
+                      Suc3_eq_add_3 Suc4_eq_add_4 add.commute)
+
+              subgoal by (cases index_reg; simp; cases base_reg; simp add: x64_decode_def bitfield_insert_u8_def Let_def ireg_of_u8_def
+                      Suc3_eq_add_3 Suc4_eq_add_4 add.commute)
+
+              subgoal by (cases index_reg; simp; cases base_reg; simp add: x64_decode_def bitfield_insert_u8_def Let_def ireg_of_u8_def
+                      Suc3_eq_add_3 Suc4_eq_add_4 add.commute)
+
+              subgoal by (cases index_reg; simp; cases base_reg; simp add: x64_decode_def bitfield_insert_u8_def Let_def ireg_of_u8_def
+                      Suc3_eq_add_3 Suc4_eq_add_4 add.commute)
+
+              subgoal by (cases index_reg; simp; cases base_reg; simp add: x64_decode_def bitfield_insert_u8_def Let_def ireg_of_u8_def
+                      Suc3_eq_add_3 Suc4_eq_add_4 add.commute)
+              done 
+            done
+        done
+      done
+    done
+  
+
+  subgoal for dst src
+    \<comment> \<open> Pmovsq_rr \<close>
+    apply (unfold Let_def construct_rex_to_u8_def construct_modsib_to_u8_def)
+    subgoal by (cases src; cases dst; auto simp add: x64_decode_def bitfield_insert_u8_def Let_def ireg_of_u8_def)
+    done
+
+  subgoal 
+    \<comment> \<open> Pcdq \<close>
+    apply(unfold Let_def x64_decode_def; simp)
+    done
+
+  subgoal 
+    \<comment> \<open> Pcqo \<close>
+    apply(unfold Let_def x64_decode_def; simp)
+    done
+
+  subgoal for dst addr
+    \<comment> \<open> Pleaq \<close>
+    apply (cases addr, simp)
+    subgoal for base index2 ofs
+      apply (cases base;simp)
+      subgoal for base_reg
+        apply (cases index2; simp add: Let_def)
+        subgoal
+          apply (erule conjE;erule conjE;erule conjE)
+          using scast_u32_scast_u8_eq
+          subgoal by (cases dst; simp;cases base_reg; simp add: construct_rex_to_u8_def  construct_modsib_to_u8_def 
+                x64_decode_def Let_def ireg_of_u8_def
+                bitfield_insert_u8_def Suc3_eq_add_3 Suc4_eq_add_4 add.commute)
+          done
+        subgoal
+          apply (erule conjE;erule conjE;erule conjE;erule conjE)
+          using list_in_list_u8_list_of_u32_simp_sym [of ofs "(Suc (Suc (Suc pc)))" l]
+          using length_u8_list_of_u32_eq_4
+          apply (cases dst; simp;cases base_reg; simp add: construct_rex_to_u8_def  construct_modsib_to_u8_def 
+                x64_decode_def Let_def ireg_of_u8_def
+                bitfield_insert_u8_def Suc3_eq_add_3 Suc4_eq_add_4 add.commute)
+          done
+        done
+      done
+    done
+
+  subgoal for dst
+    \<comment> \<open> Pnegl \<close> 
+    apply (unfold Let_def construct_rex_to_u8_def construct_modsib_to_u8_def)
+    subgoal by (cases dst; auto simp add: x64_decode_def bitfield_insert_u8_def Let_def ireg_of_u8_def)
+    done
+
+  subgoal for dst
+    \<comment> \<open> Pnegq \<close> 
+    apply (unfold Let_def construct_rex_to_u8_def construct_modsib_to_u8_def)
+    subgoal by (cases dst; auto simp add: x64_decode_def bitfield_insert_u8_def Let_def ireg_of_u8_def)
+    done 
+
+  subgoal for dst src 
+    \<comment> \<open> Paddq_rr \<close> 
+    apply (unfold Let_def construct_rex_to_u8_def construct_modsib_to_u8_def)
+    subgoal by (cases src; simp;cases dst; auto simp add: x64_decode_def bitfield_insert_u8_def Let_def ireg_of_u8_def
+          Suc3_eq_add_3 add.commute)
+    done
+
+  subgoal for dst src 
+    \<comment> \<open> Paddl_rr \<close> 
+    apply (unfold Let_def construct_rex_to_u8_def construct_modsib_to_u8_def)
+    subgoal by (cases src; cases dst; auto simp add: x64_decode_def bitfield_insert_u8_def Let_def ireg_of_u8_def)
+    done
+
+  subgoal for dst imm 
+    \<comment> \<open> Paddl_ri \<close> 
+    apply (unfold Let_def)
+    apply (cases "construct_rex_to_u8 False False False (and (u8_of_ireg dst) 8 \<noteq> 0) = 64";
+        simp_all add:construct_rex_to_u8_def construct_modsib_to_u8_def; erule conjE)
+    subgoal \<comment> \<open> rex = 0x40  \<close>
+      using list_in_list_u8_list_of_u32_simp_sym [of imm "(Suc (Suc pc))" l]
+      using length_u8_list_of_u32_eq_4
+      apply (cases dst; auto simp add: x64_decode_def bitfield_insert_u8_def Let_def
+          ireg_of_u8_def Suc3_eq_add_3 add.commute)
+      done
+
+    subgoal \<comment> \<open> rex <> 0x40  \<close>
+      using list_in_list_u8_list_of_u32_simp_sym [of imm "(pc+3)" l]
+      using length_u8_list_of_u32_eq_4
+      apply (cases dst; auto simp add: x64_decode_def bitfield_insert_u8_def Let_def
+          ireg_of_u8_def Suc3_eq_add_3 add.commute)
+      done
+    done
+
+
+  subgoal for dst imm 
+    \<comment> \<open> Paddw_ri \<close> 
+    apply (unfold Let_def)
+    apply (cases "construct_rex_to_u8 False False False (and (u8_of_ireg dst) 8 \<noteq> 0) = 64";
+        simp_all add:construct_rex_to_u8_def construct_modsib_to_u8_def; erule conjE)
+    subgoal \<comment> \<open> rex = 0x40  \<close>
+      using list_in_list_u8_list_of_u16_simp_sym [of imm " (Suc (Suc (Suc pc)))" l]
+      using length_u8_list_of_u16_eq_2
+      apply (cases dst; auto simp add: x64_decode_def bitfield_insert_u8_def Let_def
+          ireg_of_u8_def Suc3_eq_add_3 add.commute)
+      done
+
+    subgoal \<comment> \<open> rex <> 0x40  \<close>
+      using list_in_list_u8_list_of_u16_simp_sym [of imm "(Suc (Suc (Suc (Suc pc))))" l]
+      using length_u8_list_of_u16_eq_2
+      apply (cases dst; auto simp add: x64_decode_def bitfield_insert_u8_def Let_def
+          ireg_of_u8_def Suc3_eq_add_3 add.commute)
+      done
+    done
+
+
+
+  subgoal for addr imm chunk
+  \<comment> \<open> Paddq_mi \<close> 
+    apply (cases chunk, simp_all)
+    apply (cases addr)
+    subgoal for base index2 ofs
+      apply simp
+      apply (cases base, simp_all)
+      subgoal for base_reg
+        apply (cases index2, simp_all)
+        subgoal for index22
+          apply (cases index22, simp_all)
+          subgoal for index_reg scale
+            apply (erule conjE; erule conjE; erule conjE; erule conjE)
+            apply (simp add: list_in_list_concat; erule conjE)
+
+            using construct_modsib_to_u8_imply_index_reg [of "False" index_reg base_reg "l ! pc" scale "l ! Suc (Suc (Suc pc))"]
+            using construct_modsib_to_u8_imply_base_reg [of "False" index_reg base_reg "l ! pc" scale "l ! Suc (Suc (Suc pc))"]
+            using construct_modsib_to_u8_imply_scale [of scale index_reg base_reg "l ! (pc+3)"]
+            using list_in_list_u8_list_of_u32_simp_sym [of "ofs" "(pc+4)" l]
+            using length_u8_list_of_u32_eq_4
+            using list_in_list_u8_list_of_u32_simp_sym [of imm "(pc+8)" l]
+(*
+            apply (cases base_reg; simp; cases index_reg; simp add: construct_rex_to_u8_def construct_modsib_to_u8_def
+                    x64_decode_def bitfield_insert_u8_def Let_def ireg_of_u8_def
+                    add.commute Suc3_eq_add_3 Suc4_eq_add_4) *)
+            apply (cases base_reg; simp)
+            subgoal by (cases index_reg; simp add: construct_rex_to_u8_def construct_modsib_to_u8_def
+                    x64_decode_def bitfield_insert_u8_def Let_def ireg_of_u8_def
+                    add.commute Suc3_eq_add_3 Suc4_eq_add_4)
+            subgoal by (cases index_reg; simp add: construct_rex_to_u8_def construct_modsib_to_u8_def
+                    x64_decode_def bitfield_insert_u8_def Let_def ireg_of_u8_def
+                    add.commute Suc3_eq_add_3 Suc4_eq_add_4)
+            subgoal by (cases index_reg; simp add: construct_rex_to_u8_def construct_modsib_to_u8_def
+                    x64_decode_def bitfield_insert_u8_def Let_def ireg_of_u8_def
+                    add.commute Suc3_eq_add_3 Suc4_eq_add_4)
+            subgoal by (cases index_reg; simp add: construct_rex_to_u8_def construct_modsib_to_u8_def
+                    x64_decode_def bitfield_insert_u8_def Let_def ireg_of_u8_def
+                    add.commute Suc3_eq_add_3 Suc4_eq_add_4)
+            subgoal by (cases index_reg; simp add: construct_rex_to_u8_def construct_modsib_to_u8_def
+                    x64_decode_def bitfield_insert_u8_def Let_def ireg_of_u8_def
+                    add.commute Suc3_eq_add_3 Suc4_eq_add_4)
+            subgoal by (cases index_reg; simp add: construct_rex_to_u8_def construct_modsib_to_u8_def
+                    x64_decode_def bitfield_insert_u8_def Let_def ireg_of_u8_def
+                    add.commute Suc3_eq_add_3 Suc4_eq_add_4)
+            subgoal by (cases index_reg; simp add: construct_rex_to_u8_def construct_modsib_to_u8_def
+                    x64_decode_def bitfield_insert_u8_def Let_def ireg_of_u8_def
+                    add.commute Suc3_eq_add_3 Suc4_eq_add_4)
+            subgoal by (cases index_reg; simp add: construct_rex_to_u8_def construct_modsib_to_u8_def
+                    x64_decode_def bitfield_insert_u8_def Let_def ireg_of_u8_def
+                    add.commute Suc3_eq_add_3 Suc4_eq_add_4)
+            subgoal by (cases index_reg; simp add: construct_rex_to_u8_def construct_modsib_to_u8_def
+                    x64_decode_def bitfield_insert_u8_def Let_def ireg_of_u8_def
+                    add.commute Suc3_eq_add_3 Suc4_eq_add_4)
+            subgoal by (cases index_reg; simp add: construct_rex_to_u8_def construct_modsib_to_u8_def
+                    x64_decode_def bitfield_insert_u8_def Let_def ireg_of_u8_def
+                    add.commute Suc3_eq_add_3 Suc4_eq_add_4)
+            subgoal by (cases index_reg; simp add: construct_rex_to_u8_def construct_modsib_to_u8_def
+                    x64_decode_def bitfield_insert_u8_def Let_def ireg_of_u8_def
+                    add.commute Suc3_eq_add_3 Suc4_eq_add_4)
+            subgoal by (cases index_reg; simp add: construct_rex_to_u8_def construct_modsib_to_u8_def
+                    x64_decode_def bitfield_insert_u8_def Let_def ireg_of_u8_def
+                    add.commute Suc3_eq_add_3 Suc4_eq_add_4)
+            subgoal by (cases index_reg; simp add: construct_rex_to_u8_def construct_modsib_to_u8_def
+                    x64_decode_def bitfield_insert_u8_def Let_def ireg_of_u8_def
+                    add.commute Suc3_eq_add_3 Suc4_eq_add_4)
+            subgoal by (cases index_reg; simp add: construct_rex_to_u8_def construct_modsib_to_u8_def
+                    x64_decode_def bitfield_insert_u8_def Let_def ireg_of_u8_def
+                    add.commute Suc3_eq_add_3 Suc4_eq_add_4)
+            subgoal by (cases index_reg; simp add: construct_rex_to_u8_def construct_modsib_to_u8_def
+                    x64_decode_def bitfield_insert_u8_def Let_def ireg_of_u8_def
+                    add.commute Suc3_eq_add_3 Suc4_eq_add_4)
+            subgoal by (cases index_reg; simp add: construct_rex_to_u8_def construct_modsib_to_u8_def
+                    x64_decode_def bitfield_insert_u8_def Let_def ireg_of_u8_def
+                    add.commute Suc3_eq_add_3 Suc4_eq_add_4)
+            done
+          done
+        done
+      done
+    done
+
+  subgoal for dst src 
+    \<comment> \<open> Psubl_rr \<close> 
+    apply (unfold Let_def construct_rex_to_u8_def construct_modsib_to_u8_def)
+    subgoal by (cases src; cases dst; auto simp add: x64_decode_def bitfield_insert_u8_def Let_def ireg_of_u8_def)
+    done
+
+  subgoal for dst src 
+    \<comment> \<open> Psubq_rr \<close> 
+    apply (unfold Let_def construct_rex_to_u8_def construct_modsib_to_u8_def; erule conjE; erule conjE)
+    subgoal by (cases src; cases dst; auto simp add: x64_decode_def bitfield_insert_u8_def Let_def ireg_of_u8_def)
+    done
+
+  subgoal for dst imm 
+    \<comment> \<open> Psubl_ri \<close> 
+    apply (unfold Let_def)
+    apply (cases "construct_rex_to_u8 False False False (and (u8_of_ireg dst) 8 \<noteq> 0) = 64";
+        simp_all add:construct_rex_to_u8_def construct_modsib_to_u8_def; erule conjE)
+    subgoal \<comment> \<open> rex = 0x40  \<close>
+      using list_in_list_u8_list_of_u32_simp_sym [of imm "(Suc (Suc pc))" l]
+      using length_u8_list_of_u32_eq_4
+      apply (cases dst; auto simp add: x64_decode_def bitfield_insert_u8_def Let_def
+          ireg_of_u8_def Suc3_eq_add_3 add.commute)
+      done
+
+    subgoal \<comment> \<open> rex <> 0x40  \<close>
+      using list_in_list_u8_list_of_u32_simp_sym [of imm "(pc+3)" l]
+      using length_u8_list_of_u32_eq_4
+      apply (cases dst; auto simp add: x64_decode_def bitfield_insert_u8_def Let_def
+          ireg_of_u8_def Suc3_eq_add_3 add.commute)
+      done
+    done
+
+  subgoal for dst 
+    \<comment> \<open> Pmull_r \<close> 
+    apply (unfold Let_def construct_rex_to_u8_def construct_modsib_to_u8_def)
+    subgoal by (cases dst; auto simp add: x64_decode_def bitfield_insert_u8_def Let_def ireg_of_u8_def)
+    done
+
+  subgoal for dst 
+    \<comment> \<open> Pmulq_r \<close> 
+    apply (unfold Let_def construct_rex_to_u8_def construct_modsib_to_u8_def; erule conjE; erule conjE)
+    subgoal by (cases dst; auto simp add: x64_decode_def bitfield_insert_u8_def Let_def ireg_of_u8_def)
+    done
+
+  subgoal for dst 
+    \<comment> \<open> Pimull_r \<close> 
+    apply (unfold Let_def construct_rex_to_u8_def construct_modsib_to_u8_def)
+    subgoal by (cases dst; auto simp add: x64_decode_def bitfield_insert_u8_def Let_def ireg_of_u8_def)
+    done
+
+  subgoal for dst 
+    \<comment> \<open> Pimulq_r \<close> 
+    apply (unfold Let_def construct_rex_to_u8_def construct_modsib_to_u8_def; erule conjE; erule conjE)
+    subgoal by (cases dst; auto simp add: x64_decode_def bitfield_insert_u8_def Let_def ireg_of_u8_def)
+    done
+
+  subgoal for dst 
+    \<comment> \<open> Pdivl_r \<close> 
+    apply (unfold Let_def construct_rex_to_u8_def construct_modsib_to_u8_def)
+    subgoal by (cases dst; auto simp add: x64_decode_def bitfield_insert_u8_def Let_def ireg_of_u8_def)
+    done
+
+  subgoal for dst 
+    \<comment> \<open> Pdivq_r \<close> 
+    apply (unfold Let_def construct_rex_to_u8_def construct_modsib_to_u8_def; erule conjE; erule conjE)
+    subgoal by (cases dst; auto simp add: x64_decode_def bitfield_insert_u8_def Let_def ireg_of_u8_def)
+    done
+
+  subgoal for dst 
+    \<comment> \<open> Pidivl_r \<close> 
+    apply (unfold Let_def construct_rex_to_u8_def construct_modsib_to_u8_def)
+    subgoal by (cases dst; auto simp add: x64_decode_def bitfield_insert_u8_def Let_def ireg_of_u8_def)
+    done
+
+  subgoal for dst 
+    \<comment> \<open> Pidivq_r \<close> 
+    apply (unfold Let_def construct_rex_to_u8_def construct_modsib_to_u8_def; erule conjE; erule conjE)
+    subgoal by (cases dst; auto simp add: x64_decode_def bitfield_insert_u8_def Let_def ireg_of_u8_def)
+    done
+
+  subgoal for dst src 
+    \<comment> \<open> Pandl_rr \<close> 
+    apply (unfold Let_def construct_rex_to_u8_def construct_modsib_to_u8_def)
+    subgoal by (cases src; cases dst; auto simp add: x64_decode_def bitfield_insert_u8_def Let_def ireg_of_u8_def)
+    done
+
+  subgoal for dst imm 
+    \<comment> \<open> Pandl_ri\<close> 
+    apply (unfold Let_def)
+    apply (cases "construct_rex_to_u8 False False False (and (u8_of_ireg dst) 8 \<noteq> 0) = 64";
+        simp_all add:construct_rex_to_u8_def construct_modsib_to_u8_def; erule conjE)
+    subgoal \<comment> \<open> rex = 0x40  \<close>
+      using list_in_list_u8_list_of_u32_simp_sym [of imm "(Suc (Suc pc))" l]
+      using length_u8_list_of_u32_eq_4
+      apply (cases dst; auto simp add: x64_decode_def bitfield_insert_u8_def Let_def
+          ireg_of_u8_def Suc3_eq_add_3 add.commute)
+      done
+
+    subgoal \<comment> \<open> rex <> 0x40  \<close>
+      using list_in_list_u8_list_of_u32_simp_sym [of imm "(pc+3)" l]
+      using length_u8_list_of_u32_eq_4
+      apply (cases dst; auto simp add: x64_decode_def bitfield_insert_u8_def Let_def
+          ireg_of_u8_def Suc3_eq_add_3 add.commute)
+      done
+    done
+
+  subgoal for dst src
+    \<comment> \<open> Pandq_rr \<close> 
+    apply (unfold Let_def construct_rex_to_u8_def construct_modsib_to_u8_def; erule conjE; erule conjE)
+    subgoal by (cases src; cases dst; auto simp add: x64_decode_def bitfield_insert_u8_def Let_def ireg_of_u8_def)
+    done
+
+  subgoal for dst src 
+    \<comment> \<open> Porl_rr \<close> 
+    apply (unfold Let_def construct_rex_to_u8_def construct_modsib_to_u8_def)
+    subgoal by (cases src; cases dst; auto simp add: x64_decode_def bitfield_insert_u8_def Let_def ireg_of_u8_def)
+    done
+
+  subgoal for dst imm 
+    \<comment> \<open> Porl_ri\<close> 
+    apply (unfold Let_def)
+    apply (cases "construct_rex_to_u8 False False False (and (u8_of_ireg dst) 8 \<noteq> 0) = 64";
+        simp_all add:construct_rex_to_u8_def construct_modsib_to_u8_def; erule conjE)
+    subgoal \<comment> \<open> rex = 0x40  \<close>
+      using list_in_list_u8_list_of_u32_simp_sym [of imm "(Suc (Suc pc))" l]
+      using length_u8_list_of_u32_eq_4
+      apply (cases dst; auto simp add: x64_decode_def bitfield_insert_u8_def Let_def
+          ireg_of_u8_def Suc3_eq_add_3 add.commute)
+      done
+
+    subgoal \<comment> \<open> rex <> 0x40  \<close>
+      using list_in_list_u8_list_of_u32_simp_sym [of imm "(pc+3)" l]
+      using length_u8_list_of_u32_eq_4
+      apply (cases dst; auto simp add: x64_decode_def bitfield_insert_u8_def Let_def
+          ireg_of_u8_def Suc3_eq_add_3 add.commute)
+      done
+    done
+
+
+  subgoal for dst src
+    \<comment> \<open> Porq_rr \<close> 
+    apply (unfold Let_def construct_rex_to_u8_def construct_modsib_to_u8_def; erule conjE; erule conjE)
+    subgoal by (cases src; cases dst; auto simp add: x64_decode_def bitfield_insert_u8_def Let_def ireg_of_u8_def)
+    done
+
+  subgoal for dst src 
+    \<comment> \<open> Pxorl_rr \<close> 
+    apply (unfold Let_def construct_rex_to_u8_def construct_modsib_to_u8_def)
+    subgoal by (cases src; cases dst; auto simp add: x64_decode_def bitfield_insert_u8_def Let_def ireg_of_u8_def)
+    done
+
+  subgoal for dst src
+    \<comment> \<open> Pxorq_rr \<close> 
+    apply (unfold Let_def construct_rex_to_u8_def construct_modsib_to_u8_def; erule conjE; erule conjE)
+    subgoal by (cases src; cases dst; auto simp add: x64_decode_def bitfield_insert_u8_def Let_def ireg_of_u8_def)
+    done
+
+  subgoal for dst imm 
+    \<comment> \<open> Pxorl_ri\<close> 
+    apply (unfold Let_def)
+    apply (cases "construct_rex_to_u8 False False False (and (u8_of_ireg dst) 8 \<noteq> 0) = 64";
+        simp_all add:construct_rex_to_u8_def construct_modsib_to_u8_def; erule conjE)
+    subgoal \<comment> \<open> rex = 0x40  \<close>
+      using list_in_list_u8_list_of_u32_simp_sym [of imm "(Suc (Suc pc))" l]
+      using length_u8_list_of_u32_eq_4
+      apply (cases dst; auto simp add: x64_decode_def bitfield_insert_u8_def Let_def
+          ireg_of_u8_def Suc3_eq_add_3 add.commute)
+      done
+
+    subgoal \<comment> \<open> rex <> 0x40  \<close>
+      using list_in_list_u8_list_of_u32_simp_sym [of imm "(pc+3)" l]
+      using length_u8_list_of_u32_eq_4
+      apply (cases dst; auto simp add: x64_decode_def bitfield_insert_u8_def Let_def
+          ireg_of_u8_def Suc3_eq_add_3 add.commute)
+      done
+    done
+
+  
+  subgoal for dst imm
+    \<comment> \<open> Pshll_ri \<close>
+    apply (unfold Let_def)
+    apply (cases "construct_rex_to_u8 False False False (and (u8_of_ireg dst) 8 \<noteq> 0) = 64",
+        simp_all)
+
+    subgoal \<comment> \<open> rex = 0x40 \<close>
+      apply (cases dst; auto simp add: x64_decode_def bitfield_insert_u8_def Let_def ireg_of_u8_def
+          construct_rex_to_u8_def construct_modsib_to_u8_def)
+      done
+
+    subgoal  \<comment> \<open> rex <> 0x40 \<close>
+      apply (cases dst; auto simp add: x64_decode_def bitfield_insert_u8_def Let_def ireg_of_u8_def
+          construct_rex_to_u8_def construct_modsib_to_u8_def Suc3_eq_add_3 add.commute)
+      done
+    done
+
+  subgoal for dst
+    \<comment> \<open> Pshlq_ri \<close>
+    apply (unfold Let_def construct_rex_to_u8_def construct_modsib_to_u8_def; erule conjE; erule conjE)
+    apply (cases dst; auto simp add: x64_decode_def bitfield_insert_u8_def Let_def ireg_of_u8_def  Suc3_eq_add_3 add.commute)
+    done
+
+  subgoal for dst
+  \<comment> \<open> Pshll_r \<close> 
+    apply (unfold Let_def construct_rex_to_u8_def construct_modsib_to_u8_def)
+    apply (cases dst; auto simp add: x64_decode_def bitfield_insert_u8_def Let_def ireg_of_u8_def)
+    done
+
+  subgoal for dst
+  \<comment> \<open> Pshlq_r \<close> 
+    apply (unfold Let_def construct_rex_to_u8_def construct_modsib_to_u8_def)
+    apply (cases dst; auto simp add: x64_decode_def bitfield_insert_u8_def Let_def ireg_of_u8_def)
+    done
+
+  subgoal for dst imm
+    \<comment> \<open> Pshrl_ri \<close>
+    apply (unfold Let_def)
+    apply (cases "construct_rex_to_u8 False False False (and (u8_of_ireg dst) 8 \<noteq> 0) = 64",
+        simp_all)
+
+    subgoal \<comment> \<open> rex = 0x40 \<close>
+      apply (cases dst; auto simp add: x64_decode_def bitfield_insert_u8_def Let_def ireg_of_u8_def
+          construct_rex_to_u8_def construct_modsib_to_u8_def)
+      done
+
+    subgoal  \<comment> \<open> rex <> 0x40 \<close>
+      apply (cases dst; auto simp add: x64_decode_def bitfield_insert_u8_def Let_def ireg_of_u8_def
+          construct_rex_to_u8_def construct_modsib_to_u8_def Suc3_eq_add_3 add.commute)
+      done
+    done
+
+  subgoal for dst
+    \<comment> \<open> Pshrq_ri \<close>
+    apply (unfold Let_def construct_rex_to_u8_def construct_modsib_to_u8_def; erule conjE; erule conjE)
+    apply (cases dst; auto simp add: x64_decode_def bitfield_insert_u8_def Let_def ireg_of_u8_def  Suc3_eq_add_3 add.commute)
+    done
+
+
+  subgoal for dst
+  \<comment> \<open> Pshrl_r \<close> 
+    apply (unfold Let_def construct_rex_to_u8_def construct_modsib_to_u8_def)
+    apply (cases dst; auto simp add: x64_decode_def bitfield_insert_u8_def Let_def ireg_of_u8_def)
+    done     
+
+  subgoal for dst
+  \<comment> \<open> Pshrq_r \<close> 
+    apply (unfold Let_def construct_rex_to_u8_def construct_modsib_to_u8_def)
+    apply (cases dst; auto simp add: x64_decode_def bitfield_insert_u8_def Let_def ireg_of_u8_def)
+    done
+
+  subgoal for dst imm
+    \<comment> \<open> Psarl_ri \<close>
+    apply (unfold Let_def construct_rex_to_u8_def construct_modsib_to_u8_def)
+    apply (cases dst; auto simp add: x64_decode_def bitfield_insert_u8_def Let_def ireg_of_u8_def  Suc3_eq_add_3 add.commute)
+    done
+
+  subgoal for dst
+  \<comment> \<open> Psarq_ri \<close> 
+    apply (unfold Let_def construct_rex_to_u8_def construct_modsib_to_u8_def; erule conjE; erule conjE)
+    apply (cases dst; auto simp add: x64_decode_def bitfield_insert_u8_def Let_def ireg_of_u8_def  Suc3_eq_add_3 add.commute)
+    done
+
+  subgoal for dst
+  \<comment> \<open> Psarl_r \<close> 
+    apply (unfold Let_def construct_rex_to_u8_def construct_modsib_to_u8_def)
+    apply (cases dst; auto simp add: x64_decode_def bitfield_insert_u8_def Let_def ireg_of_u8_def)
+    done  
+
+  subgoal for dst
+  \<comment> \<open> Psarq_r \<close> 
+    apply (unfold Let_def construct_rex_to_u8_def construct_modsib_to_u8_def)
+    apply (cases dst; auto simp add: x64_decode_def bitfield_insert_u8_def Let_def ireg_of_u8_def)
+    done  
+
+  subgoal for dst imm
+    \<comment> \<open> Prolw_ri \<close>
+    apply (unfold Let_def)
+    apply (cases "construct_rex_to_u8 False False False (and (u8_of_ireg dst) 8 \<noteq> 0) = 64",
+        simp_all)
+
+    subgoal \<comment> \<open> rex = 0x40 \<close>
+      apply (cases dst; auto simp add: x64_decode_def bitfield_insert_u8_def Let_def ireg_of_u8_def
+          construct_rex_to_u8_def construct_modsib_to_u8_def Suc3_eq_add_3 add.commute)
+      done
+
+    subgoal  \<comment> \<open> rex <> 0x40 \<close>
+      apply (cases dst; auto simp add: x64_decode_def bitfield_insert_u8_def Let_def ireg_of_u8_def
+          construct_rex_to_u8_def construct_modsib_to_u8_def Suc3_eq_add_3 add.commute)
+      done
+    done
+
+  subgoal for dst
+    \<comment> \<open> Pbswapl \<close> 
+    apply (unfold Let_def construct_rex_to_u8_def construct_modsib_to_u8_def)
+    subgoal by (cases dst; auto simp add: x64_decode_def bitfield_insert_u8_def Let_def ireg_of_u8_def)
+    done
+
+  subgoal for dst
+    \<comment> \<open> Pbswapq \<close> 
+    apply (unfold Let_def construct_rex_to_u8_def construct_modsib_to_u8_def)
+    subgoal by (cases dst; auto simp add: x64_decode_def bitfield_insert_u8_def Let_def ireg_of_u8_def)
+    done
+
+  subgoal for dst
+    \<comment> \<open> Ppushl_r \<close> 
+    apply (unfold Let_def construct_rex_to_u8_def construct_modsib_to_u8_def)
+    subgoal by (cases dst; auto simp add: x64_decode_def bitfield_insert_u8_def Let_def ireg_of_u8_def)
+    done
+
+  subgoal for imm
+    \<comment> \<open> Ppushl_i \<close> 
+    apply (unfold Let_def construct_rex_to_u8_def construct_modsib_to_u8_def)
+    subgoal 
+      using list_in_list_u8_list_of_u32_simp_sym [of imm  "(Suc (Suc pc))" l]
+      using length_u8_list_of_u32_eq_4
+      apply(auto simp add: x64_decode_def bitfield_insert_u8_def Let_def ireg_of_u8_def Suc3_eq_add_3 add.commute)
+      done
+    done
+
+  subgoal for addr chunk 
+    \<comment> \<open> Ppushq_m \<close> 
+    apply (cases chunk,simp_all)
+    apply (cases addr, simp_all)
+    subgoal for base index2 ofs
+      apply (cases base;simp)
+      subgoal for base_reg
+        apply (cases index2; simp add: Let_def)
+        subgoal for index22
+          apply (cases index22, simp_all)
+          subgoal for index_reg scale
+            apply (erule conjE;erule conjE;erule conjE;erule conjE)
+            using list_in_list_u8_list_of_u32_simp_sym [of ofs "(Suc (Suc (Suc (Suc pc))))" l]
+            using length_u8_list_of_u32_eq_4
+            using construct_modsib_to_u8_imply_index_reg [of "False" index_reg base_reg "l ! pc" scale "l ! Suc (Suc (Suc pc))"]
+            using construct_modsib_to_u8_imply_base_reg [of "False" index_reg base_reg "l ! pc" scale "l ! Suc (Suc (Suc pc))"]
+            using construct_modsib_to_u8_imply_scale [of scale index_reg base_reg "l ! Suc (Suc (Suc pc))"]
+            subgoal by(cases base_reg; simp; cases index_reg; simp add: 
+                  construct_rex_to_u8_def construct_modsib_to_u8_def
+                    x64_decode_def bitfield_insert_u8_def Let_def ireg_of_u8_def
+                    add.commute Suc3_eq_add_3 Suc4_eq_add_4)
+            done
+          done
+        done
+      done
+    done
+
+  subgoal for dst
+    \<comment> \<open> Ppopl_i \<close> 
+    apply (unfold Let_def construct_rex_to_u8_def construct_modsib_to_u8_def)
+    apply (cases dst; auto simp add: x64_decode_def bitfield_insert_u8_def Let_def ireg_of_u8_def)
+    done
+
+  subgoal for dst src
+    \<comment> \<open> Ptestl_rr \<close>
+    apply (unfold Let_def construct_rex_to_u8_def construct_modsib_to_u8_def)
+    subgoal by (cases src; cases dst; auto simp add: x64_decode_def bitfield_insert_u8_def Let_def ireg_of_u8_def)
+    done
+
+  subgoal for dst src
+    \<comment> \<open> Ptestq_rr \<close>
+    apply (unfold Let_def construct_rex_to_u8_def construct_modsib_to_u8_def)
+    subgoal by (cases src; cases dst; auto simp add: x64_decode_def bitfield_insert_u8_def Let_def ireg_of_u8_def)
+    done
+
+  subgoal for dst imm
+  \<comment> \<open> Ptestl_ri  \<close>
+    apply (unfold Let_def)
+    apply (cases "construct_rex_to_u8 False False False (and (u8_of_ireg dst) 8 \<noteq> 0) = 64";
+        simp_all add:construct_rex_to_u8_def construct_modsib_to_u8_def; erule conjE)
+    subgoal \<comment> \<open> rex = 0x40  \<close>
+      using list_in_list_u8_list_of_u32_simp_sym [of imm "(Suc (Suc pc))" l]
+      using length_u8_list_of_u32_eq_4
+      apply (cases dst; auto simp add: x64_decode_def bitfield_insert_u8_def Let_def
+          ireg_of_u8_def Suc3_eq_add_3 add.commute)
+      done
+
+    subgoal \<comment> \<open> rex <> 0x40  \<close>
+      using list_in_list_u8_list_of_u32_simp_sym [of imm "(pc+3)" l]
+      using length_u8_list_of_u32_eq_4
+      apply (cases dst; auto simp add: x64_decode_def bitfield_insert_u8_def Let_def
+          ireg_of_u8_def Suc3_eq_add_3 add.commute)
+      done
+    done
+
+  subgoal for dst imm
+  \<comment> \<open> Ptestq_ri  \<close>
+    apply (unfold Let_def construct_rex_to_u8_def construct_modsib_to_u8_def)
+    using list_in_list_u8_list_of_u32_simp_sym [of imm "(Suc (Suc (Suc pc)))" l]
+    using length_u8_list_of_u32_eq_4
+    apply (cases dst; simp_all add: bitfield_insert_u8_def x64_decode_def ireg_of_u8_def Suc3_eq_add_3 add.commute)
+    done
+
+  subgoal for dst src
+    \<comment> \<open> Pcmpl_rr \<close>
+    apply (unfold Let_def construct_rex_to_u8_def construct_modsib_to_u8_def)
+    subgoal by (cases src; cases dst; auto simp add: x64_decode_def bitfield_insert_u8_def Let_def ireg_of_u8_def)
+    done
+
+  subgoal for dst src
+    \<comment> \<open> Pcmpq_rr \<close>
+    apply (unfold Let_def construct_rex_to_u8_def construct_modsib_to_u8_def;  erule conjE; erule conjE)
+    subgoal by (cases src; cases dst; auto simp add: x64_decode_def bitfield_insert_u8_def Let_def ireg_of_u8_def)
+    done
+
+  subgoal for dst imm
+  \<comment> \<open> Pcmpl_ri  \<close>
+    apply (unfold Let_def)
+    apply (cases "construct_rex_to_u8 False False False (and (u8_of_ireg dst) 8 \<noteq> 0) = 64";
+        simp_all add:construct_rex_to_u8_def construct_modsib_to_u8_def; erule conjE)
+    subgoal \<comment> \<open> rex = 0x40  \<close>
+      using list_in_list_u8_list_of_u32_simp_sym [of imm "(Suc (Suc pc))" l]
+      using length_u8_list_of_u32_eq_4
+      apply (cases dst; auto simp add: x64_decode_def bitfield_insert_u8_def Let_def
+          ireg_of_u8_def Suc3_eq_add_3 add.commute)
+      done
+
+    subgoal \<comment> \<open> rex <> 0x40  \<close>
+      using list_in_list_u8_list_of_u32_simp_sym [of imm "(pc+3)" l]
+      using length_u8_list_of_u32_eq_4
+      apply (cases dst; auto simp add: x64_decode_def bitfield_insert_u8_def Let_def
+          ireg_of_u8_def Suc3_eq_add_3 add.commute)
+      done
+    done
+
+  subgoal for dst imm
+  \<comment> \<open> Pcmpq_ri\<close>
+    apply (unfold Let_def construct_rex_to_u8_def construct_modsib_to_u8_def; erule conjE; erule conjE; erule conjE)
+    using list_in_list_u8_list_of_u32_simp_sym [of imm "(Suc (Suc (Suc pc)))" l]
+    using length_u8_list_of_u32_eq_4
+    apply (cases dst; simp_all add: bitfield_insert_u8_def x64_decode_def ireg_of_u8_def Suc3_eq_add_3 add.commute)
+    done
+
+  subgoal for test imm
+    \<comment> \<open> Pjcc \<close>
+    subgoal 
+      using list_in_list_u8_list_of_u32_simp_sym [of imm "(Suc (Suc pc))" l]
+      using length_u8_list_of_u32_eq_4
+      apply (cases test; auto simp add: x64_decode_def bitfield_insert_u8_def Let_def ireg_of_u8_def
+             cond_of_u8_def Suc3_eq_add_3 add.commute)
+      done
+    done
+
+  subgoal for imm
+    \<comment> \<open> Pjmp \<close>
+    subgoal 
+      using list_in_list_u8_list_of_u32_simp_sym [of imm "(Suc pc)" l]
+      using length_u8_list_of_u32_eq_4
+      apply (auto simp add: x64_decode_def bitfield_insert_u8_def Let_def ireg_of_u8_def
+            Suc3_eq_add_3 add.commute)
+      done
+    done
+
+  subgoal for dst 
+    \<comment> \<open> Pcall_r \<close> 
+    apply (unfold Let_def construct_rex_to_u8_def construct_modsib_to_u8_def)
+    subgoal by (cases dst; auto simp add: x64_decode_def bitfield_insert_u8_def Let_def ireg_of_u8_def)
+    done
+
+  subgoal for imm 
+    \<comment> \<open> Pcall_i \<close> 
+    subgoal 
+      using list_in_list_u8_list_of_u32_simp_sym [of imm "(Suc pc)" l]
+      using length_u8_list_of_u32_eq_4
+      apply (auto simp add: x64_decode_def bitfield_insert_u8_def Let_def ireg_of_u8_def
+            Suc3_eq_add_3 add.commute)
+      done
+    done
+
+  subgoal 
+    \<comment> \<open> Pret \<close>
+    apply(unfold Let_def x64_decode_def; simp)
+    done
+
+  subgoal 
+    \<comment> \<open> Prdtsc \<close>
+    apply(unfold Let_def x64_decode_def; simp)
+    done
+
+  subgoal 
+    \<comment> \<open> Pnop \<close>
+    apply(unfold Let_def x64_decode_def; simp)
+    done
   done
+
+declare if_split_asm [split del]
 end
